step_simulation almost complete.

compcomp/InliningproofEFF.v
@@ -62,7 +62,7 @@ Lemma function_ptr_translated:
     Genv.find_funct_ptr ge b = Some f ->
     exists f', Genv.find_funct_ptr tge b = Some f' /\ transf_fundef fenv f = OK f'.
 Proof.
-eapply (Genv.find_funct_ptr_transf_partial (transf_fundef fenv) _ TRANSF).
+  eapply (Genv.find_funct_ptr_transf_partial (transf_fundef fenv) _ TRANSF).
 Qed.
 Lemma sig_function_translated:
   forall f f', transf_fundef fenv f = OK f' ->  funsig f' =  funsig f.
@@ -228,7 +228,7 @@ Lemma tr_moves_init_regs:
                                    list_forall2 (val_reg_charact F ctx1 rs1) vl rsrcs ->
                                    exists rs2,
                                      star  step tge (State stk f sp pc1 rs1 m)
-                                          E0 (State stk f sp pc2 rs2 m)
+                                           E0 (State stk f sp pc2 rs2 m)
                                      /\ agree_regs F ctx2 (init_regs vl rdsts) rs2
                                      /\ forall r, Plt r ctx2.(dreg) -> rs2#r = rs1#r.
 Proof.
@@ -391,21 +391,21 @@ Proof.
   eapply function_ptr_translated; eauto.
 Qed.
 
-(** ** Relating stacks *)
-
+(** ** Relating stacks *) 
 Inductive match_stacks (mu: SM_Injection) (m m': mem):
   list stackframe -> list stackframe -> block -> Prop :=
 | match_stacks_nil: forall bound1 bound
                            (MG: match_globalenvs (as_inj mu) bound1)
-                           (BELOW: Ple bound1 bound),
+                           (BELOW: Ple bound1 bound)
+                           (* SL: locBlockSrc mu bound = true *),
                       match_stacks mu m m' nil nil bound
 | match_stacks_cons: forall res (f:function) sp pc rs stk (f':function) sp' rs' stk' bound ctx
                             (MS: match_stacks_inside mu m m' stk stk' f' ctx sp' rs')
                             (FB: tr_funbody fenv f'.(fn_stacksize) ctx f f'.(fn_code))
                             (AG: agree_regs (as_inj mu) ctx rs rs')
                             (SP: (as_inj mu) sp = Some(sp', ctx.(dstk)))
-(*locBlockSrc mu sp = true*)
-(*locBlockTrg mu sp' = true*)
+(* locBlockSrc mu sp = true *)
+(SL: locBlocksTgt mu sp' = true )
 (PRIV: range_private (as_inj mu) m m' sp' (ctx.(dstk) + ctx.(mstk)) f'.(fn_stacksize))
 (SSZ1: 0 <= f'.(fn_stacksize) < Int.max_unsigned)
 (SSZ2: forall ofs, Mem.perm m' sp' ofs Max Nonempty -> 0 <= ofs <= f'.(fn_stacksize))
@@ -421,7 +421,7 @@ Inductive match_stacks (mu: SM_Injection) (m m': mem):
                                   (SSZ1: 0 <= f'.(fn_stacksize) < Int.max_unsigned)
                                   (SSZ2: forall ofs, Mem.perm m' sp' ofs Max Nonempty -> 0 <= ofs <= f'.(fn_stacksize))
                                   (RET: ctx.(retinfo) = Some (rpc, res))
-(*locBlockTrg mu sp' = true*)
+(SL: locBlocksTgt mu sp' = true )
 (BELOW: Plt sp' bound),
                              match_stacks (mu) m m'
                                           stk
@@ -432,7 +432,7 @@ with match_stacks_inside (mu: SM_Injection) (m m': mem):
        list stackframe -> list stackframe -> function -> context -> block -> regset -> Prop :=
      | match_stacks_inside_base: forall stk stk' f' ctx sp' rs'
                                         (MS: match_stacks (mu) m m' stk stk' sp')
-(*locBlockTrg mu sp' = true*)(*Maybe*)
+(SL: locBlocksTgt mu sp' = true ) (*Maybe*)
 (RET: ctx.(retinfo) = None)
 (DSTK: ctx.(dstk) = 0),
                                    match_stacks_inside (mu) m m' stk stk' f' ctx sp' rs'
@@ -440,9 +440,9 @@ with match_stacks_inside (mu: SM_Injection) (m m': mem):
                                            (MS: match_stacks_inside (mu) m m' stk stk' f' ctx' sp' rs')
                                            (FB: tr_funbody fenv f'.(fn_stacksize) ctx' f f'.(fn_code))
                                            (AG: agree_regs (as_inj mu) ctx' rs rs')
-                                           (SP: (as_inj mu) sp = Some(sp', ctx'.(dstk)))
+                                           (SP: (local_of mu) sp = Some(sp', ctx'.(dstk)))
 (*locBlockSrc mu sp = true*)
-(*locBlockTrg mu sp' = true*)
+(SL: locBlocksTgt mu sp' = true )
 (PAD: range_private (as_inj mu) m m' sp' (ctx'.(dstk) + ctx'.(mstk)) ctx.(dstk))
 (RES: Ple res ctx'.(mreg))
 (RET: ctx.(retinfo) = Some (spc ctx' pc, sreg ctx' res))
@@ -501,7 +501,18 @@ Section MATCH_STACKS.
   Variable F1: SM_Injection.
   Let Finj1 := as_inj F1.
   Variables m1 m1': mem.
-  Hypothesis INCR: inject_incr Finj Finj1.
+  (*Hypothesis INCR: inject_incr Finj Finj1.*)
+  Hypothesis INCR: intern_incr F F1.
+  Hypothesis WDF: SM_wd F.
+  Hypothesis WDF1: SM_wd F1.
+  Lemma INCR':  inject_incr Finj Finj1.
+    eapply intern_incr_as_inj; auto.
+  Qed.
+  Lemma incre_local_of: forall mu mu' (INCR0: intern_incr mu mu') b b' delta, local_of mu b = Some (b', delta) -> local_of mu' b = Some (b', delta).
+      intros.
+      apply intern_incr_local in INCR0.
+      apply INCR0; auto.
+  Qed.
 
   Lemma match_stacks_invariant:
     forall stk stk' bound, match_stacks F m m' stk stk' bound ->
@@ -533,6 +544,7 @@ Section MATCH_STACKS.
                                         match_stacks_inside F1 m1 m1' stk stk' f' ctx sp' rs2.
 
   Proof.
+    assert (INCR':  inject_incr Finj Finj1) by (exact INCR').
     induction 1; intros.
     (* nil *)
     apply match_stacks_nil with (bound1 := bound1).
@@ -547,6 +559,7 @@ Section MATCH_STACKS.
     intros; eapply PERM2; eauto; xomega.
     intros; eapply PERM3; eauto; xomega.
     eapply agree_regs_incr; eauto.
+    destruct INCR; repeat open_Hyp; apply H2; assumption.
     eapply range_private_invariant; eauto. 
     (* untailcall *)
     apply match_stacks_untailcall with (ctx := ctx); auto. 
@@ -556,7 +569,8 @@ Section MATCH_STACKS.
     intros; eapply PERM2; eauto; xomega.
     intros; eapply PERM3; eauto; xomega.
     eapply range_private_invariant; eauto. 
-
+    destruct INCR; repeat open_Hyp; apply H2; assumption.
+    assert (INCR':  inject_incr Finj Finj1) by (exact INCR').
     induction 1; intros.
     (* base *)
     eapply match_stacks_inside_base; eauto.
@@ -565,13 +579,16 @@ Section MATCH_STACKS.
     intros; eapply PERM1; eauto; xomega.
     intros; eapply PERM2; eauto; xomega.
     intros; eapply PERM3; eauto; xomega.
+    destruct INCR; repeat open_Hyp; apply H2; assumption.
     (* inlined *)
     apply match_stacks_inside_inlined with (ctx' := ctx'); auto. 
     apply IHmatch_stacks_inside; auto.
     intros. apply RS. red in BELOW. xomega. 
     apply agree_regs_incr with Finj; auto. 
     apply agree_regs_invariant with rs'; auto. 
-    intros. apply RS. red in BELOW. xomega. 
+    intros. apply RS. red in BELOW. xomega.
+    eapply (incre_local_of F F1); auto.
+    destruct INCR; repeat open_Hyp. apply H3; assumption.
     eapply range_private_invariant; eauto.
     intros. split. eapply INJ; eauto. xomega. eapply PERM1; eauto. xomega.
     intros. eapply PERM2; eauto. xomega.
@@ -598,9 +615,11 @@ End MATCH_STACKS.
 
 
 (** Preservation by assignment to a register *)
+Hint Immediate intern_incr_refl. (* : incr_refl.*)
 
 Lemma match_stacks_inside_set_reg:
-  forall F m m' stk stk' f' ctx sp' rs' r v, 
+  forall F m m' stk stk' f' ctx sp' rs' r v,
+    SM_wd F ->
     match_stacks_inside F m m' stk stk' f' ctx sp' rs' ->
     match_stacks_inside F m m' stk stk' f' ctx sp' (rs'#(sreg ctx r) <- v).
 Proof.
@@ -612,6 +631,7 @@ Qed.
 
 Lemma match_stacks_inside_store:
   forall F m m' stk stk' f' ctx sp' rs' chunk b ofs v m1 chunk' b' ofs' v' m1', 
+    SM_wd F ->
     match_stacks_inside F m m' stk stk' f' ctx sp' rs' ->
     Mem.store chunk m b ofs v = Some m1 ->
     Mem.store chunk' m' b' ofs' v' = Some m1' ->
@@ -625,38 +645,47 @@ Qed.
 
 Lemma match_stacks_inside_alloc_left:
   forall F m m' stk stk' f' ctx sp' rs',
+    SM_wd F ->
     match_stacks_inside F m m' stk stk' f' ctx sp' rs' ->
     forall sz m1 b F1 delta,
+    SM_wd F1 ->
       Mem.alloc m 0 sz = (m1, b) ->
-      inject_incr (as_inj F) (as_inj F1) ->
+      (intern_incr F F1) ->
       (as_inj F1) b = Some(sp', delta) ->
       (forall b1, b1 <> b -> (as_inj F1) b1 = (as_inj F) b1) ->
       delta >= ctx.(dstk) ->
       match_stacks_inside F1 m1 m' stk stk' f' ctx sp' rs'.
 Proof.
-  induction 1; intros.
+  induction 2; intros.
   (* base *)
-  eapply match_stacks_inside_base; eauto. 
-  eapply match_stacks_invariant; eauto.
+  eapply match_stacks_inside_base; eauto.
+  eapply (match_stacks_invariant F m m' F1); eauto.
   intros. destruct (eq_block b1 b).
-  subst b1. rewrite H1 in H4; inv H4. eelim Plt_strict; eauto. 
-  rewrite H2 in H4; auto. 
+  subst b1. rewrite H3 in H6; inv H6. eelim Plt_strict; eauto. 
+  rewrite H4 in H6; auto. 
   intros. exploit Mem.perm_alloc_inv; eauto. destruct (eq_block b1 b); intros; auto.
-  subst b1. rewrite H1 in H4. inv H4. eelim Plt_strict; eauto. 
+  subst b1. rewrite H3 in H6; inv H6. eelim Plt_strict; eauto. 
+  destruct H2; repeat open_Hyp. apply H8; assumption.
   (* inlined *)
+  assert (INCR':  inject_incr (as_inj F) (as_inj F1)).
+  eapply intern_incr_as_inj; auto.
   eapply match_stacks_inside_inlined; eauto. 
   eapply IHmatch_stacks_inside; eauto. destruct SBELOW. omega. 
   eapply agree_regs_incr; eauto.
+  apply intern_incr_local in H3.
+  apply H3; auto.
+  destruct H3; repeat open_Hyp. apply H9; assumption.
   eapply range_private_invariant; eauto. 
   intros. exploit Mem.perm_alloc_inv; eauto. destruct (eq_block b0 b); intros.
-  subst b0. rewrite H2 in H5; inv H5. elimtype False; xomega. 
-  rewrite H3 in H5; auto. 
+  subst b0. rewrite H4 in H7; inv H7. elimtype False; xomega. 
+  rewrite H5 in H7; auto. 
 Qed.
 
 (** Preservation by freeing *)
 
 Lemma match_stacks_free_left:
   forall F m m' stk stk' sp b lo hi m1,
+    SM_wd F ->
     match_stacks F m m' stk stk' sp ->
     Mem.free m b lo hi = Some m1 ->
     match_stacks F m1 m' stk stk' sp.
@@ -667,6 +696,7 @@ Qed.
 
 Lemma match_stacks_free_right:
   forall F m m' stk stk' sp lo hi m1',
+    SM_wd F ->
     match_stacks F m m' stk stk' sp ->
     Mem.free m' sp lo hi = Some m1' ->
     match_stacks F m m1' stk stk' sp.
@@ -707,6 +737,8 @@ Qed.
 Section EXTCALL.
 
   Variables F1 F2: SM_Injection.
+  Hypothesis WDF1: SM_wd F1.
+  Hypothesis WDF2: SM_wd F2.
   Let Finj1 := as_inj F1.
   Let Finj2 := as_inj F2.
   Variables m1 m2 m1' m2': mem.
@@ -714,7 +746,9 @@ Section EXTCALL.
   Hypothesis MAXPERM': forall b ofs p, Mem.valid_block m1' b -> Mem.perm m2' b ofs Max p -> Mem.perm m1' b ofs Max p.
   Hypothesis UNCHANGED: Mem.unchanged_on (loc_out_of_reach Finj1 m1) m1' m2'.
   Hypothesis INJ: Mem.inject Finj1 m1 m1'.
-  Hypothesis INCR: inject_incr Finj1 Finj2.
+  Hypothesis INCR: intern_incr F1 F2.
+  (* Hypothesis INCR: inject_incr Finj1 Finj2. *)
+  About INCR'.
   Hypothesis SEP: inject_separated Finj1 Finj2 m1 m1'.
 
   Lemma match_stacks_extcall:
@@ -728,27 +762,34 @@ Section EXTCALL.
                Plt sp' (Mem.nextblock m1') ->
                match_stacks_inside F2 m2 m2' stk stk' f' ctx sp' rs'.
   Proof.
+    assert (INCR': inject_incr Finj1 Finj2) by (apply INCR'; auto). 
     induction 1; intros.
     apply match_stacks_nil with bound1; auto. 
     inv MG. constructor; intros; eauto. 
     destruct (Finj1 b1) as [[b2' delta']|] eqn:?.
-    exploit INCR; eauto. intros EQ; unfold Finj2 in EQ; rewrite H0 in EQ; inv EQ.
+    exploit INCR'; eauto. intros EQ; unfold Finj2 in EQ; rewrite H0 in EQ; inv EQ.
     eapply IMAGE; eauto. 
     exploit SEP; eauto. intros [A B]. elim B. red. xomega. 
     eapply match_stacks_cons; eauto. 
     eapply match_stacks_inside_extcall; eauto. xomega. 
     eapply agree_regs_incr; eauto. 
+    destruct INCR; repeat open_Hyp. apply H3; assumption.
     eapply range_private_extcall; eauto. red; xomega. 
     intros. apply SSZ2; auto. apply MAXPERM'; auto. red; xomega.
     eapply match_stacks_untailcall; eauto. 
     eapply match_stacks_inside_extcall; eauto. xomega. 
     eapply range_private_extcall; eauto. red; xomega. 
     intros. apply SSZ2; auto. apply MAXPERM'; auto. red; xomega.
+    destruct INCR; repeat open_Hyp; apply H3; assumption.
+    assert (INCR': inject_incr Finj1 Finj2) by (apply INCR'; auto). 
     induction 1; intros.
     eapply match_stacks_inside_base; eauto.
     eapply match_stacks_extcall; eauto. xomega. 
+    destruct INCR; repeat open_Hyp; apply H3; assumption.
     eapply match_stacks_inside_inlined; eauto. 
-    eapply agree_regs_incr; eauto. 
+    eapply agree_regs_incr; eauto.    
+    eapply (incre_local_of F1); auto.
+    destruct INCR; repeat open_Hyp; apply H4; assumption.
     eapply range_private_extcall; eauto.
   Qed.
 
@@ -844,7 +885,7 @@ Inductive match_states:  SM_Injection -> RTL_core -> mem -> RTL_core -> mem -> P
 Print REACH_closed.
 About REACH.
 Definition MATCH (d:RTL_core) mu c1 m1 c2 m2:Prop :=
-  match_states mu c1 m1 c2 m2 /\
+  match_states (restrict_sm mu (vis mu)) c1 m1 c2 m2 /\
   REACH_closed m1 (vis mu) /\
   meminj_preserves_globals ge (as_inj mu) /\
   (forall b, isGlobalBlock ge b = true -> frgnBlocksSrc mu b = true) /\
@@ -855,9 +896,9 @@ Definition MATCH (d:RTL_core) mu c1 m1 c2 m2:Prop :=
 (** ** Forward simulation *)
 Definition RTL_measure (S: RTL_core) : nat :=
   match S with
-  | RTL_State _ _ _ _ _ => 1%nat
-  | RTL_Callstate _ _ _ => 0%nat
-  | RTL_Returnstate _ _ => 0%nat
+    | RTL_State _ _ _ _ _ => 1%nat
+    | RTL_Callstate _ _ _ => 0%nat
+    | RTL_Returnstate _ _ => 0%nat
   end.
 
 
@@ -872,12 +913,14 @@ Qed.
 
 
 Definition entry_points_ok entrypoints:= forall (v1 v2 : val) (sig : signature),
-                                             In (v1, v2, sig) entrypoints -> 
-                                             exists b f1 f2, 
-                                               v1 = Vptr b Int.zero 
-                                               /\ v2 = Vptr b Int.zero
-                                               /\ Genv.find_funct_ptr ge b = Some f1
-                                               /\ Genv.find_funct_ptr tge b = Some f2.
+                                           In (v1, v2, sig) entrypoints -> 
+                                           exists b f1 f2, 
+                                             v1 = Vptr b Int.zero 
+                                             /\ v2 = Vptr b Int.zero
+                                             /\ Genv.find_funct_ptr ge b = Some f1
+                                             /\ Genv.find_funct_ptr tge b = Some f2.
+
+
 
 (** ** Behold the theorem *)
 Theorem transl_program_correct:
@@ -894,7 +937,7 @@ Theorem transl_program_correct:
   eapply sepcomp.effect_simulations_lemmas.inj_simulation_star with (match_states:= MATCH)(measure:= RTL_measure).
 
   Lemma environment_equality: (exists m0:mem, Genv.init_mem SrcProg = Some m0) -> 
-                                     genvs_domain_eq ge tge.
+                              genvs_domain_eq ge tge.
     descend;
     destruct H0 as [b0]; exists b0;
     rewriter_back;
@@ -917,365 +960,367 @@ Theorem transl_program_correct:
   eauto with trans_correct.
 
 
-Lemma MATCH_restrict: forall (d : RTL_core) (mu : SM_Injection) (c1 : RTL_core) 
-                                 (m1 : mem) (c2 : RTL_core) (m2 : mem) (X : block -> bool) (MC: MATCH d mu c1 m1 c2 m2)(HX: forall b : block, vis mu b = true -> X b = true)(RC0:REACH_closed m1 X), MATCH d (restrict_sm mu X) c1 m1 c2 m2.
-intros.
-Proof. intros.
-  destruct MC as [MC [RC [PG [GF [VAL [WDmu [INJ GFP]]]]]]].
-assert (WDR: SM_wd (restrict_sm mu X)).
-   apply restrict_sm_WD; assumption.
+  Lemma MATCH_restrict: forall (d : RTL_core) (mu : SM_Injection) (c1 : RTL_core) 
+                               (m1 : mem) (c2 : RTL_core) (m2 : mem) (X : block -> bool) (MC: MATCH d mu c1 m1 c2 m2)(HX: forall b : block, vis mu b = true -> X b = true)(RC0:REACH_closed m1 X), MATCH d (restrict_sm mu X) c1 m1 c2 m2.
+    intros.
+    destruct MC as [MC [RC [PG [GF [VAL [WDmu INJ]]]]]].
+    assert (WDR: SM_wd (restrict_sm mu X)).
+    apply restrict_sm_WD; assumption.
+    split; try rewrite vis_restrict_sm; try rewrite restrict_sm_all; try rewrite restrict_sm_frgnBlocksSrc.
+    rewrite restrict_sm_nest; assumption.
+    intuition.
 
-split.
+    (*meminj_preserves_globals*)
+    rewrite <- restrict_sm_all.
+    eapply restrict_sm_preserves_globals; auto.
+    intros.
+    apply HX.
+    unfold vis.
+    rewrite GF; auto. 
+    apply orb_true_r.
 
-Lemma match_states_restrict: forall mu m1 m2 c1 c2 X
-      (HX: forall b, vis mu b = true -> X b = true)
-      (RC: REACH_closed m1 X)
-      (MCS: match_states mu c1 m1 c2 m2 ),
-      match_states (restrict_sm mu X) c1 m1 c2 m2.
-  admit.
-Qed.
+    (* sm_valid  *)
+    unfold sm_valid; split; intros;
+    red in VAL; destruct VAL as [H0 H1].
+    apply H0; unfold DOM; erewrite <- restrict_sm_DomSrc; eauto.
+    apply H1; unfold RNG; erewrite <- restrict_sm_DomTgt; eauto.
+    
+    (*  Mem.inject *)
+    SearchAbout Mem.inject restrict.
+    apply inject_restrict; try assumption.
+  Qed.
 
-apply match_states_restrict; intuition.
+  Hint Resolve MATCH_restrict: trans_correct.
+  auto with trans_correct.
 
-split. unfold vis.
-  rewrite restrict_sm_locBlocksSrc, restrict_sm_frgnBlocksSrc.
-  apply RC.
-split. (*clear -PG HX.*)
-  eapply restrict_sm_preserves_globals; try eassumption.
-  unfold vis in HX. intuition.
-split. 
-  rewrite restrict_sm_frgnBlocksSrc. apply GF.
-split.
-destruct VAL.
-(*This should be a lemma*)
-unfold sm_valid.
-    rewrite restrict_sm_DOM.
-    rewrite restrict_sm_RNG.
-    split; intros; intuition.
-split. assumption.
-(*split.*)
- rewrite restrict_sm_all.
-eapply  inject_restrict; repeat (first [assumption| split]).
-Qed.
-Hint Resolve MATCH_restrict: trans_correct.
-auto with trans_correct.
-
-Lemma MATCH_valid:  forall (d : RTL_core) (mu : SM_Injection) (c1 : RTL_core) 
-                              (m1 : mem) (c2 : RTL_core) (m2 : mem)
-                         (MC: MATCH d mu c1 m1 c2 m2), sm_valid mu m1 m2.
-intros.
-apply MC.
-Qed.
-
-Hint Resolve MATCH_valid: trans_correct.
-eauto with trans_correct.
-
-Lemma MATCH_PG:  forall (d : RTL_core) (mu : SM_Injection) (c1 : RTL_core) 
-                                           (m1 : mem) (c2 : RTL_core) (m2 : mem)(
-                                      MC: MATCH d mu c1 m1 c2 m2),
-                                      meminj_preserves_globals ge (extern_of mu) /\
-                                      (forall b : block,
-                                         isGlobalBlock ge b = true -> frgnBlocksSrc mu b = true).
-Proof.
-  intros.
-  assert (GF: forall b, isGlobalBlock ge b = true -> frgnBlocksSrc mu b = true).
+  Lemma MATCH_valid:  forall (d : RTL_core) (mu : SM_Injection) (c1 : RTL_core) 
+                             (m1 : mem) (c2 : RTL_core) (m2 : mem)
+                             (MC: MATCH d mu c1 m1 c2 m2), sm_valid mu m1 m2.
+    intros.
     apply MC.
-  split; trivial.
-  rewrite <- match_genv_meminj_preserves_extern_iff_all; trivial.
+  Qed.
+
+  Hint Resolve MATCH_valid: trans_correct.
+  eauto with trans_correct.
+
+  Lemma MATCH_PG:  forall (d : RTL_core) (mu : SM_Injection) (c1 : RTL_core) 
+                          (m1 : mem) (c2 : RTL_core) (m2 : mem)(
+                            MC: MATCH d mu c1 m1 c2 m2),
+                     meminj_preserves_globals ge (extern_of mu) /\
+                     (forall b : block,
+                        isGlobalBlock ge b = true -> frgnBlocksSrc mu b = true).
+  Proof.
+    intros.
+    assert (GF: forall b, isGlobalBlock ge b = true -> frgnBlocksSrc mu b = true).
+    apply MC.
+    split; trivial.
+    rewrite <- match_genv_meminj_preserves_extern_iff_all; trivial.
     apply MC. apply MC.
-Qed.
-Hint Resolve MATCH_PG: trans_correct.
-eauto with trans_correct.
+  Qed.
+  Hint Resolve MATCH_PG: trans_correct.
+  eauto with trans_correct.
 
-Lemma MATCH_initial_core: forall (v1 v2 : val) (sig : signature) entrypoints
-  (entry_ok : entry_points_ok entrypoints)
-   (EP: In (v1, v2, sig) entrypoints)
-   (vals1 : list val) (c1 : RTL_core) (m1 : mem) 
-     (j : meminj) (vals2 : list val) (m2 : mem) (DomS DomT : block -> bool)
-   (SM_Ini:initial_core rtl_eff_sem ge v1 vals1 = Some c1)
-   (Inj: Mem.inject j m1 m2)
-   (VInj: Forall2 (val_inject j) vals1 vals2)
-   (PG: meminj_preserves_globals ge j)
-   (J: forall (b1 b2 : block) (d : Z),
-    j b1 = Some (b2, d) -> DomS b1 = true /\ DomT b2 = true)
-   (RCH: forall b : block,
-    REACH m2 (fun b' : block => isGlobalBlock tge b' || getBlocks vals2 b')
-      b = true -> DomT b = true)
-   (HDomS: (forall b : block, DomS b = true -> Mem.valid_block m1 b))
-   (HDomT: (forall b : block, DomT b = true -> Mem.valid_block m2 b)),
-   exists c2 : RTL_core,
-     initial_core rtl_eff_sem tge v2 vals2 = Some c2 /\
-     MATCH c1
-       (initial_SM DomS DomT
-          (REACH m1
-             (fun b : block => isGlobalBlock ge b || getBlocks vals1 b))
-          (REACH m2
-             (fun b : block => isGlobalBlock tge b || getBlocks vals2 b)) j)
-       c1 m1 c2 m2.
- Proof.
-  intros.
-  inversion SM_Ini.
-  unfold  RTL_initial_core in H0. unfold ge in *. unfold tge in *.
-  destruct v1; inv H0.
-  remember (Int.eq_dec i Int.zero) as z; destruct z; inv H1. clear Heqz.
-  remember (Genv.find_funct_ptr (Genv.globalenv SrcProg) b) as zz; destruct zz; inv H0. 
+  Lemma MATCH_initial_core: forall (v1 v2 : val) (sig : signature) entrypoints
+                                   (entry_ok : entry_points_ok entrypoints)
+                                   (EP: In (v1, v2, sig) entrypoints)
+                                   (vals1 : list val) (c1 : RTL_core) (m1 : mem) 
+                                   (j : meminj) (vals2 : list val) (m2 : mem) (DomS DomT : block -> bool)
+                                   (SM_Ini:initial_core rtl_eff_sem ge v1 vals1 = Some c1)
+                                   (Inj: Mem.inject j m1 m2)
+                                   (VInj: Forall2 (val_inject j) vals1 vals2)
+                                   (PG: meminj_preserves_globals ge j)
+                                   (J: forall (b1 b2 : block) (d : Z),
+                                         j b1 = Some (b2, d) -> DomS b1 = true /\ DomT b2 = true)
+                                   (RCH: forall b : block,
+                                           REACH m2 (fun b' : block => isGlobalBlock tge b' || getBlocks vals2 b')
+                                                 b = true -> DomT b = true)
+                                   (HDomS: (forall b : block, DomS b = true -> Mem.valid_block m1 b))
+                                   (HDomT: (forall b : block, DomT b = true -> Mem.valid_block m2 b)),
+                            exists c2 : RTL_core,
+                              initial_core rtl_eff_sem tge v2 vals2 = Some c2 /\
+                              MATCH c1
+                                    (initial_SM DomS DomT
+                                                (REACH m1
+                                                       (fun b : block => isGlobalBlock ge b || getBlocks vals1 b))
+                                                (REACH m2
+                                                       (fun b : block => isGlobalBlock tge b || getBlocks vals2 b)) j)
+                                    c1 m1 c2 m2.
+  Proof.
+    intros.
+    inversion SM_Ini.
+    unfold  RTL_initial_core in H0. unfold ge in *. unfold tge in *.
+    destruct v1; inv H0.
+    remember (Int.eq_dec i Int.zero) as z; destruct z; inv H1. clear Heqz.
+    remember (Genv.find_funct_ptr (Genv.globalenv SrcProg) b) as zz; destruct zz; inv H0. 
     apply eq_sym in Heqzz.
-  exploit function_ptr_translated; eauto. intros [tf [FIND TR]].
-  exists (RTL_Callstate nil tf vals2).
-  split. 
-  simpl. 
-  destruct (entry_ok _ _ _ EP) as [b0 [f1 [f2 [A [B [C D]]]]]].
-  subst. inv A.
-  unfold ge, tge in *. rewrite C in Heqzz. inv Heqzz. 
-  rewrite D in FIND. inv FIND.
-  unfold RTL_initial_core. 
-  case_eq (Int.eq_dec Int.zero Int.zero). intros ? e.
-  solve[rewrite D; auto].
-  intros CONTRA.
-  solve[elimtype False; auto].
-  admit.
-Qed.
-Hint Resolve MATCH_initial_core: trans_correct.
-eauto with trans_correct.
+    exploit function_ptr_translated; eauto. intros [tf [FIND TR]].
+    exists (RTL_Callstate nil tf vals2).
+    split. 
+    simpl. 
+    destruct (entry_ok _ _ _ EP) as [b0 [f1 [f2 [A [B [C D]]]]]].
+    subst. inv A.
+    unfold ge, tge in *. rewrite C in Heqzz. inv Heqzz. 
+    rewrite D in FIND. inv FIND.
+    unfold RTL_initial_core. 
+    case_eq (Int.eq_dec Int.zero Int.zero). intros ? e.
+    solve[rewrite D; auto].
+    intros CONTRA.
+    solve[elimtype False; auto].
+    admit.
+  Qed.
+  Hint Resolve MATCH_initial_core: trans_correct.
+  eauto with trans_correct.
 
-Lemma Match_Halted: forall (cd : RTL_core) (mu : SM_Injection) (c1 : RTL_core) 
-     (m1 : mem) (c2 : RTL_core) (m2 : mem) (v1 : val)(MC:
-   MATCH cd mu c1 m1 c2 m2)(HALT:
-   halted rtl_eff_sem c1 = Some v1),
-   exists v2 : val,
-     Mem.inject (as_inj mu) m1 m2 /\
-     val_inject (restrict (as_inj mu) (vis mu)) v1 v2 /\
-     halted rtl_eff_sem c2 = Some v2.
-Proof.
-intros.
-unfold MATCH in MC; destruct MC as [H0 H1].
-inv H0; simpl in *; inv HALT. 
-Print match_states.
-inv MS. 
-exists v'; split; try assumption; split; try reflexivity; inv H0. admit.
-inv H0.
-inv MS0; [rewrite RET in RET0; inv RET0 | inv H0].
-inv MS.
-rewrite RET in RET0; inv RET0.
-inv H0.
-Qed.
-Hint Resolve Match_Halted: trans_correct.
-eauto with trans_correct.
+  Lemma Match_Halted: forall (cd : RTL_core) (mu : SM_Injection) (c1 : RTL_core) 
+                             (m1 : mem) (c2 : RTL_core) (m2 : mem) (v1 : val)(MC:
+                                                                                MATCH cd mu c1 m1 c2 m2)(HALT:
+                                                                                                           halted rtl_eff_sem c1 = Some v1),
+                      exists v2 : val,
+                        Mem.inject (as_inj mu) m1 m2 /\
+                        val_inject (restrict (as_inj mu) (vis mu)) v1 v2 /\
+                        halted rtl_eff_sem c2 = Some v2.
+  Proof.
+    intros.
+    unfold MATCH in MC; destruct MC as [H0 H1].
+    inv H0; simpl in *; inv HALT. 
+    Print match_states.
+    inv MS. 
+    exists v'; split; try assumption. eapply H1.
 
-Lemma at_external_lemma: forall (mu : SM_Injection) (c1 : RTL_core) (m1 : mem) 
-                                (c2 : RTL_core) (m2 : mem) (e : external_function) 
-                                (vals1 : list val) (ef_sig : signature)(MC: MATCH c1 mu c1 m1 c2 m2) (ATE: at_external rtl_eff_sem c1 = Some (e, ef_sig, vals1)),
-                           Mem.inject (as_inj mu) m1 m2 /\ 
-                           (exists vals2 : list val, Forall2 (val_inject (restrict (as_inj mu) (vis mu))) vals1 vals2 /\ at_external rtl_eff_sem c2 = Some (e, ef_sig, vals2)).
-  intros.
-  split. inv MC; apply H0.
-  inv MC; simpl in *. inv H; inv ATE.
-  destruct fd; inv H1.
-  exists args'.
-  split. apply val_list_inject_forall_inject. admit.
-  inv FD; trivial.
-Qed.
-Hint Resolve at_external_lemma: trans_correct.
-eauto with trans_correct.
+    inv H0.
+    split; trivial.
+    rewrite <- restrict_sm_all; assumption.
+    inv H0.
+    inv MS0.
+    rewrite RET in RET0; inv RET0.
+    inv H0.
+    inv MS.
+    rewrite RET in RET0; inv RET0.
+    inv H0.
+  Qed.
+  Hint Resolve Match_Halted: trans_correct.
+  eauto with trans_correct.
 
-Lemma Match_AfterExternal: 
-forall (mu : SM_Injection) (st1 : RTL_core) (st2 : RTL_core) (m1 : mem) (e : external_function) (vals1 : list val) (m2 : mem) (ef_sig : signature) (vals2 : list val) (e' : external_function) (ef_sig' : signature) 
-       (MemInjMu : Mem.inject (as_inj mu) m1 m2)
-       (MatchMu : MATCH st1 mu st1 m1 st2 m2)
-       (AtExtSrc : at_external rtl_eff_sem st1 = Some (e, ef_sig, vals1))
-       (AtExtTgt : at_external rtl_eff_sem st2 = Some (e', ef_sig', vals2))
-       (ValInjMu : Forall2 (val_inject (restrict (as_inj mu) (vis mu))) vals1 vals2)
-       (pubSrc' : block -> bool)
-       (pubSrcHyp : pubSrc' =
-              (fun b : block =>
-               locBlocksSrc mu b && REACH m1 (exportedSrc mu vals1) b))
-       (pubTgt' : block -> bool)
-       (pubTgtHyp : pubTgt' =
-              (fun b : block =>
-               locBlocksTgt mu b && REACH m2 (exportedTgt mu vals2) b))
-       (nu : SM_Injection)
-       (NuHyp : nu = replace_locals mu pubSrc' pubTgt')
-       (nu' : SM_Injection)
-       (ret1 : val)
-       (m1' : mem)
-       (ret2 : val)
-       (m2' : mem)
-       (INC : extern_incr nu nu')
-       (SEP : sm_inject_separated nu nu' m1 m2)
-       (WDnu' : SM_wd nu')
-       (SMvalNu' : sm_valid nu' m1' m2')
-       (MemInjNu' : Mem.inject (as_inj nu') m1' m2')
-       (RValInjNu' : val_inject (as_inj nu') ret1 ret2)
-       (FwdSrc : mem_forward m1 m1')
-       (FwdTgt : mem_forward m2 m2')
-       (frgnSrc' : block -> bool)
-       (frgnSrcHyp : frgnSrc' =
-               (fun b : block =>
-                DomSrc nu' b &&
-                (negb (locBlocksSrc nu' b) &&
-                 REACH m1' (exportedSrc nu' (ret1 :: nil)) b)))
-       (frgnTgt' : block -> bool)
-       (frgnTgtHyp : frgnTgt' =
-               (fun b : block =>
-                DomTgt nu' b &&
-                (negb (locBlocksTgt nu' b) &&
-                 REACH m2' (exportedTgt nu' (ret2 :: nil)) b)))
-       (mu' : SM_Injection)
-       (Mu'Hyp : mu' = replace_externs nu' frgnSrc' frgnTgt')
-       (UnchPrivSrc : Mem.unchanged_on
-                  (fun (b : block) (_ : Z) =>
-                   locBlocksSrc nu b = true /\ pubBlocksSrc nu b = false) m1 m1')
-       (UnchLOOR : Mem.unchanged_on (local_out_of_reach nu m1) m2 m2'),
-exists (st1' st2' : RTL_core),
-  after_external rtl_eff_sem (Some ret1) st1 = Some st1' /\
-  after_external rtl_eff_sem (Some ret2) st2 = Some st2' /\
-  MATCH st1' mu' st1' m1' st2' m2'.
-Proof. intros. 
- destruct MatchMu as [MC [RC [PG [GF [VAL [WDmu [INJ GFP]]]]]]].
- inv MC; simpl in *; inv AtExtSrc.
-  destruct fd; inv H0.
-  destruct fd'; inv AtExtTgt.
-  exists (RTL_Returnstate stk ret1). eexists.
-    split. reflexivity.
-    split. reflexivity.
-  simpl in *.
-inv FD.
-assert (INCvisNu': inject_incr
-  (restrict (as_inj nu')
-     (vis
-        (replace_externs nu'
-           (fun b : Values.block =>
-            DomSrc nu' b &&
-            (negb (locBlocksSrc nu' b) &&
-             REACH m1' (exportedSrc nu' (ret1 :: nil)) b))
-           (fun b : Values.block =>
-            DomTgt nu' b &&
-            (negb (locBlocksTgt nu' b) &&
-             REACH m2' (exportedTgt nu' (ret2 :: nil)) b))))) (as_inj nu')).
-      unfold vis. rewrite replace_externs_frgnBlocksSrc, replace_externs_locBlocksSrc.
-      apply restrict_incr. 
-assert (RC': REACH_closed m1' (mapped (as_inj nu'))).
-        eapply inject_REACH_closed; eassumption.
-assert (PHnu': meminj_preserves_globals (Genv.globalenv SrcProg) (as_inj nu')).
-    subst. clear - INC SEP PG GF WDmu WDnu'.
-    apply meminj_preserves_genv2blocks in PG.
-    destruct PG as [PGa [PGb PGc]].
-    apply meminj_preserves_genv2blocks.
-    split; intros.
-      specialize (PGa _ H).
-      apply joinI; left. apply INC.
-      rewrite replace_locals_extern.
-      apply foreign_in_extern.
-     assert (GG: isGlobalBlock ge b = true).
-          unfold isGlobalBlock, ge. apply genv2blocksBool_char1 in H.
-          rewrite H. trivial.
-      Check frgnSrc.
-      destruct (frgnSrc _ WDmu _ (GF _ GG)) as [bb2 [dd [FF FT2]]].
-      rewrite (foreign_in_all _ _ _ _ FF) in PGa. inv PGa.
-      assumption.
-    split; intros. specialize (PGb _ H).
-      apply joinI; left. apply INC.
-      rewrite replace_locals_extern. 
-      assert (GG: isGlobalBlock ge b = true). (*4 goals*)
-          unfold isGlobalBlock, ge. apply genv2blocksBool_char2 in H.
-          rewrite H. intuition. (*3 goals*)
-      destruct (frgnSrc _ WDmu _ (GF _ GG)) as [bb2 [dd [FF FT2]]].
-      rewrite (foreign_in_all _ _ _ _ FF) in PGb. inv PGb.
-      apply foreign_in_extern; eassumption. (*2 goals*)
-    eapply (PGc _ _ delta H). specialize (PGb _ H). clear PGa PGc.
-      remember (as_inj mu b1) as d.
-      destruct d; apply eq_sym in Heqd. (*3 goals*)
-        destruct p. 
-        apply extern_incr_as_inj in INC; trivial. (*3 goals*)
-        rewrite replace_locals_as_inj in INC.
-        rewrite (INC _ _ _ Heqd) in H0. trivial. (*3 goals*)
-      destruct SEP as [SEPa _].
-        rewrite replace_locals_as_inj, replace_locals_DomSrc, replace_locals_DomTgt in SEPa. 
-        destruct (SEPa _ _ _ Heqd H0).
-        destruct (as_inj_DomRng _ _ _ _ PGb WDmu).
-        congruence. (*1 goal*)
-assert (RR1: REACH_closed m1'
-  (fun b : Values.block =>
-   locBlocksSrc nu' b
-   || DomSrc nu' b &&
-      (negb (locBlocksSrc nu' b) &&
-       REACH m1' (exportedSrc nu' (ret1 :: nil)) b))).
-  intros b Hb. rewrite REACHAX in Hb. destruct Hb as [L HL].
-  generalize dependent b.
-  induction L; simpl; intros; inv HL.
-     assumption.
-  specialize (IHL _ H1); clear H1.
-  apply orb_true_iff in IHL.
-  remember (locBlocksSrc nu' b') as l.
-  destruct l; apply eq_sym in Heql.
-  (*case locBlocksSrc nu' b' = true*)
-    clear IHL.
-    remember (pubBlocksSrc nu' b') as p.
-    destruct p; apply eq_sym in Heqp.
-      assert (Rb': REACH m1' (mapped (as_inj nu')) b' = true).
-        apply REACH_nil. 
-        destruct (pubSrc _ WDnu' _ Heqp) as [bb2 [dd1 [PUB PT]]].
-        eapply mappedI_true.
+  (* The rewriters *)
+  Hint Rewrite vis_restrict_sm: restrict.
+  Hint Rewrite restrict_sm_all: restrict.
+  Hint Rewrite restrict_sm_frgnBlocksSrc: restrict.
+
+  Lemma at_external_lemma: forall (mu : SM_Injection) (c1 : RTL_core) (m1 : mem) 
+                                  (c2 : RTL_core) (m2 : mem) (e : external_function) 
+                                  (vals1 : list val) (ef_sig : signature)(MC: MATCH c1 mu c1 m1 c2 m2) (ATE: at_external rtl_eff_sem c1 = Some (e, ef_sig, vals1)),
+                             Mem.inject (as_inj mu) m1 m2 /\ 
+                             (exists vals2 : list val, Forall2 (val_inject (restrict (as_inj mu) (vis mu))) vals1 vals2 /\ at_external rtl_eff_sem c2 = Some (e, ef_sig, vals2)).
+    intros.
+    split. inv MC; apply H0.
+    inv MC; simpl in *. inv H; inv ATE.
+    destruct fd; inv H1.
+    exists args'.
+    split. apply val_list_inject_forall_inject.
+    autorewrite with restrict in VINJ; assumption.
+    inv FD; trivial.
+  Qed.
+  Hint Resolve at_external_lemma: trans_correct.
+  eauto with trans_correct.
+
+  Lemma Match_AfterExternal: 
+    forall (mu : SM_Injection) (st1 : RTL_core) (st2 : RTL_core) (m1 : mem) (e : external_function) (vals1 : list val) (m2 : mem) (ef_sig : signature) (vals2 : list val) (e' : external_function) (ef_sig' : signature) 
+           (MemInjMu : Mem.inject (as_inj mu) m1 m2)
+           (MatchMu : MATCH st1 mu st1 m1 st2 m2)
+           (AtExtSrc : at_external rtl_eff_sem st1 = Some (e, ef_sig, vals1))
+           (AtExtTgt : at_external rtl_eff_sem st2 = Some (e', ef_sig', vals2))
+           (ValInjMu : Forall2 (val_inject (restrict (as_inj mu) (vis mu))) vals1 vals2)
+           (pubSrc' : block -> bool)
+           (pubSrcHyp : pubSrc' =
+                        (fun b : block =>
+                           locBlocksSrc mu b && REACH m1 (exportedSrc mu vals1) b))
+           (pubTgt' : block -> bool)
+           (pubTgtHyp : pubTgt' =
+                        (fun b : block =>
+                           locBlocksTgt mu b && REACH m2 (exportedTgt mu vals2) b))
+           (nu : SM_Injection)
+           (NuHyp : nu = replace_locals mu pubSrc' pubTgt')
+           (nu' : SM_Injection)
+           (ret1 : val)
+           (m1' : mem)
+           (ret2 : val)
+           (m2' : mem)
+           (INC : extern_incr nu nu')
+           (SEP : sm_inject_separated nu nu' m1 m2)
+           (WDnu' : SM_wd nu')
+           (SMvalNu' : sm_valid nu' m1' m2')
+           (MemInjNu' : Mem.inject (as_inj nu') m1' m2')
+           (RValInjNu' : val_inject (as_inj nu') ret1 ret2)
+           (FwdSrc : mem_forward m1 m1')
+           (FwdTgt : mem_forward m2 m2')
+           (frgnSrc' : block -> bool)
+           (frgnSrcHyp : frgnSrc' =
+                         (fun b : block =>
+                            DomSrc nu' b &&
+                                   (negb (locBlocksSrc nu' b) &&
+                                         REACH m1' (exportedSrc nu' (ret1 :: nil)) b)))
+           (frgnTgt' : block -> bool)
+           (frgnTgtHyp : frgnTgt' =
+                         (fun b : block =>
+                            DomTgt nu' b &&
+                                   (negb (locBlocksTgt nu' b) &&
+                                         REACH m2' (exportedTgt nu' (ret2 :: nil)) b)))
+           (mu' : SM_Injection)
+           (Mu'Hyp : mu' = replace_externs nu' frgnSrc' frgnTgt')
+           (UnchPrivSrc : Mem.unchanged_on
+                            (fun (b : block) (_ : Z) =>
+                               locBlocksSrc nu b = true /\ pubBlocksSrc nu b = false) m1 m1')
+           (UnchLOOR : Mem.unchanged_on (local_out_of_reach nu m1) m2 m2'),
+    exists (st1' st2' : RTL_core),
+      after_external rtl_eff_sem (Some ret1) st1 = Some st1' /\
+      after_external rtl_eff_sem (Some ret2) st2 = Some st2' /\
+      MATCH st1' mu' st1' m1' st2' m2'.
+  Proof. intros. 
+         destruct MatchMu as [MC [RC [PG [GF [VAL [WDmu [INJ GFP]]]]]]].
+         inv MC; simpl in *; inv AtExtSrc.
+         destruct fd; inv H0.
+         destruct fd'; inv AtExtTgt.
+         exists (RTL_Returnstate stk ret1). eexists.
+         split. reflexivity.
+         split. reflexivity.
+         simpl in *.
+         inv FD.
+         assert (INCvisNu': inject_incr
+                              (restrict (as_inj nu')
+                                        (vis
+                                           (replace_externs nu'
+                                                            (fun b : Values.block =>
+                                                               DomSrc nu' b &&
+                                                                      (negb (locBlocksSrc nu' b) &&
+                                                                            REACH m1' (exportedSrc nu' (ret1 :: nil)) b))
+                                                            (fun b : Values.block =>
+                                                               DomTgt nu' b &&
+                                                                      (negb (locBlocksTgt nu' b) &&
+                                                                            REACH m2' (exportedTgt nu' (ret2 :: nil)) b))))) (as_inj nu')).
+         unfold vis. rewrite replace_externs_frgnBlocksSrc, replace_externs_locBlocksSrc.
+         apply restrict_incr. 
+         assert (RC': REACH_closed m1' (mapped (as_inj nu'))).
+         eapply inject_REACH_closed; eassumption.
+         assert (PHnu': meminj_preserves_globals (Genv.globalenv SrcProg) (as_inj nu')).
+         subst. clear - INC SEP PG GF WDmu WDnu'.
+         apply meminj_preserves_genv2blocks in PG.
+         destruct PG as [PGa [PGb PGc]].
+         apply meminj_preserves_genv2blocks.
+         split; intros.
+         specialize (PGa _ H).
+         apply joinI; left. apply INC.
+         rewrite replace_locals_extern.
+         apply foreign_in_extern.
+         assert (GG: isGlobalBlock ge b = true).
+         unfold isGlobalBlock, ge. apply genv2blocksBool_char1 in H.
+         rewrite H. trivial.
+         Check frgnSrc.
+         destruct (frgnSrc _ WDmu _ (GF _ GG)) as [bb2 [dd [FF FT2]]].
+         rewrite (foreign_in_all _ _ _ _ FF) in PGa. inv PGa.
+         assumption.
+         split; intros. specialize (PGb _ H).
+         apply joinI; left. apply INC.
+         rewrite replace_locals_extern. 
+         assert (GG: isGlobalBlock ge b = true). (*4 goals*)
+         unfold isGlobalBlock, ge. apply genv2blocksBool_char2 in H.
+         rewrite H. intuition. (*3 goals*)
+         destruct (frgnSrc _ WDmu _ (GF _ GG)) as [bb2 [dd [FF FT2]]].
+         rewrite (foreign_in_all _ _ _ _ FF) in PGb. inv PGb.
+         apply foreign_in_extern; eassumption. (*2 goals*)
+         eapply (PGc _ _ delta H). specialize (PGb _ H). clear PGa PGc.
+         remember (as_inj mu b1) as d.
+         destruct d; apply eq_sym in Heqd. (*3 goals*)
+         destruct p. 
+         apply extern_incr_as_inj in INC; trivial. (*3 goals*)
+         rewrite replace_locals_as_inj in INC.
+         rewrite (INC _ _ _ Heqd) in H0. trivial. (*3 goals*)
+         destruct SEP as [SEPa _].
+         rewrite replace_locals_as_inj, replace_locals_DomSrc, replace_locals_DomTgt in SEPa. 
+         destruct (SEPa _ _ _ Heqd H0).
+         destruct (as_inj_DomRng _ _ _ _ PGb WDmu).
+         congruence. (*1 goal*)
+         assert (RR1: REACH_closed m1'
+                                   (fun b : Values.block =>
+                                      locBlocksSrc nu' b
+                                                   || DomSrc nu' b &&
+                                                   (negb (locBlocksSrc nu' b) &&
+                                                         REACH m1' (exportedSrc nu' (ret1 :: nil)) b))).
+         intros b Hb. rewrite REACHAX in Hb. destruct Hb as [L HL].
+         generalize dependent b.
+         induction L; simpl; intros; inv HL.
+         assumption.
+         specialize (IHL _ H1); clear H1.
+         apply orb_true_iff in IHL.
+         remember (locBlocksSrc nu' b') as l.
+         destruct l; apply eq_sym in Heql.
+         (*case locBlocksSrc nu' b' = true*)
+         clear IHL.
+         remember (pubBlocksSrc nu' b') as p.
+         destruct p; apply eq_sym in Heqp.
+         assert (Rb': REACH m1' (mapped (as_inj nu')) b' = true).
+         apply REACH_nil. 
+         destruct (pubSrc _ WDnu' _ Heqp) as [bb2 [dd1 [PUB PT]]].
+         eapply mappedI_true.
          apply (pub_in_all _ WDnu' _ _ _ PUB).
-      assert (Rb:  REACH m1' (mapped (as_inj nu')) b = true).
-        eapply REACH_cons; try eassumption.
-      specialize (RC' _ Rb).
-      destruct (mappedD_true _ _ RC') as [[b2 d1] AI'].
-      remember (locBlocksSrc nu' b) as d.
-      destruct d; simpl; trivial.
-      apply andb_true_iff. 
-      split. eapply as_inj_DomRng; try eassumption.
-      eapply REACH_cons; try eassumption.
-        apply REACH_nil. unfold exportedSrc.
-        rewrite (pubSrc_shared _ WDnu' _ Heqp). intuition.
-      destruct (UnchPrivSrc) as [UP UV]; clear UnchLOOR.
-        specialize (UP b' z Cur Readable). 
-        specialize (UV b' z). 
-        destruct INC as [_ [_ [_ [_ [LCnu' [_ [PBnu' [_ [FRGnu' _]]]]]]]]].
-        rewrite <- LCnu'. rewrite replace_locals_locBlocksSrc.  
-        rewrite <- LCnu' in Heql. rewrite replace_locals_locBlocksSrc in *.
-        rewrite <- PBnu' in Heqp. rewrite replace_locals_pubBlocksSrc in *.
-        clear INCvisNu'. 
-        rewrite Heql in *. simpl in *. intuition.
-        assert (VB: Mem.valid_block m1 b').
-          eapply VAL. unfold DOM, DomSrc. rewrite Heql. intuition.
-        apply (H VB) in H2.
-        rewrite (H0 H2) in H4. clear H H0.
-        remember (locBlocksSrc mu b) as q.
-        destruct q; simpl; trivial; apply eq_sym in Heqq.
-        assert (Rb : REACH m1 (vis mu) b = true).
-           eapply REACH_cons; try eassumption.
-           apply REACH_nil. unfold vis. rewrite Heql; trivial.
-        specialize (RC _ Rb). unfold vis in RC.
-           rewrite Heqq in RC; simpl in *.
-        rewrite replace_locals_frgnBlocksSrc in FRGnu'.
-        rewrite FRGnu' in RC.
-        apply andb_true_iff.  
-        split. unfold DomSrc. rewrite (frgnBlocksSrc_extBlocksSrc _ WDnu' _ RC). intuition.
-        apply REACH_nil. unfold exportedSrc.
-          rewrite (frgnSrc_shared _ WDnu' _ RC). intuition.
-  (*case DomSrc nu' b' &&
+         assert (Rb:  REACH m1' (mapped (as_inj nu')) b = true).
+         eapply REACH_cons; try eassumption.
+         specialize (RC' _ Rb).
+         destruct (mappedD_true _ _ RC') as [[b2 d1] AI'].
+         remember (locBlocksSrc nu' b) as d.
+         destruct d; simpl; trivial.
+         apply andb_true_iff. 
+         split. eapply as_inj_DomRng; try eassumption.
+         eapply REACH_cons; try eassumption.
+         apply REACH_nil. unfold exportedSrc.
+         rewrite (pubSrc_shared _ WDnu' _ Heqp). intuition.
+         destruct (UnchPrivSrc) as [UP UV]; clear UnchLOOR.
+         specialize (UP b' z Cur Readable). 
+         specialize (UV b' z). 
+         destruct INC as [_ [_ [_ [_ [LCnu' [_ [PBnu' [_ [FRGnu' _]]]]]]]]].
+         rewrite <- LCnu'. rewrite replace_locals_locBlocksSrc.  
+         rewrite <- LCnu' in Heql. rewrite replace_locals_locBlocksSrc in *.
+         rewrite <- PBnu' in Heqp. rewrite replace_locals_pubBlocksSrc in *.
+         clear INCvisNu'. 
+         rewrite Heql in *. simpl in *. intuition.
+         assert (VB: Mem.valid_block m1 b').
+         eapply VAL. unfold DOM, DomSrc. rewrite Heql. intuition.
+         apply (H VB) in H2.
+         rewrite (H0 H2) in H4. clear H H0.
+         remember (locBlocksSrc mu b) as q.
+         destruct q; simpl; trivial; apply eq_sym in Heqq.
+         assert (Rb : REACH m1 (vis mu) b = true).
+         eapply REACH_cons; try eassumption.
+         apply REACH_nil. unfold vis. rewrite Heql; trivial.
+         specialize (RC _ Rb). unfold vis in RC.
+         rewrite Heqq in RC; simpl in *.
+         rewrite replace_locals_frgnBlocksSrc in FRGnu'.
+         rewrite FRGnu' in RC.
+         apply andb_true_iff.  
+         split. unfold DomSrc. rewrite (frgnBlocksSrc_extBlocksSrc _ WDnu' _ RC). intuition.
+         apply REACH_nil. unfold exportedSrc.
+         rewrite (frgnSrc_shared _ WDnu' _ RC). intuition.
+         (*case DomSrc nu' b' &&
     (negb (locBlocksSrc nu' b') &&
      REACH m1' (exportedSrc nu' (ret1 :: nil)) b') = true*)
-    destruct IHL. inv H.
-    apply andb_true_iff in H. simpl in H. 
-    destruct H as[DomNu' Rb']. 
-    clear INC SEP INCvisNu' UnchLOOR UnchPrivSrc.
-    remember (locBlocksSrc nu' b) as d.
-    destruct d; simpl; trivial. apply eq_sym in Heqd.
-    apply andb_true_iff.
-    split. assert (RET: Forall2 (val_inject (as_inj nu')) (ret1::nil) (ret2::nil)).
-              constructor. assumption. constructor.
-           destruct (REACH_as_inj _ WDnu' _ _ _ _ MemInjNu' RET
-               _ Rb' (fun b => true)) as [b2 [d1 [AI' _]]]; trivial.
-           assert (REACH m1' (mapped (as_inj nu')) b = true).
-             eapply REACH_cons; try eassumption.
-             apply REACH_nil. eapply mappedI_true; eassumption.
-           specialize (RC' _ H). 
-           destruct (mappedD_true _ _ RC') as [[? ?] ?].
-           eapply as_inj_DomRng; eassumption.
-    eapply REACH_cons; try eassumption.
-(*assert (RRR: REACH_closed m1' (exportedSrc nu' (ret1 :: nil))).
+         destruct IHL. inv H.
+         apply andb_true_iff in H. simpl in H. 
+         destruct H as[DomNu' Rb']. 
+         clear INC SEP INCvisNu' UnchLOOR UnchPrivSrc.
+         remember (locBlocksSrc nu' b) as d.
+         destruct d; simpl; trivial. apply eq_sym in Heqd.
+         apply andb_true_iff.
+         split. assert (RET: Forall2 (val_inject (as_inj nu')) (ret1::nil) (ret2::nil)).
+         constructor. assumption. constructor.
+         destruct (REACH_as_inj _ WDnu' _ _ _ _ MemInjNu' RET
+                                _ Rb' (fun b => true)) as [b2 [d1 [AI' _]]]; trivial.
+         assert (REACH m1' (mapped (as_inj nu')) b = true).
+         eapply REACH_cons; try eassumption.
+         apply REACH_nil. eapply mappedI_true; eassumption.
+         specialize (RC' _ H). 
+         destruct (mappedD_true _ _ RC') as [[? ?] ?].
+         eapply as_inj_DomRng; eassumption.
+         eapply REACH_cons; try eassumption.
+         (*assert (RRR: REACH_closed m1' (exportedSrc nu' (ret1 :: nil))).
     intros b Hb. apply REACHAX in Hb.
        destruct Hb as [L HL].
        generalize dependent b.
@@ -1284,49 +1329,51 @@ assert (RR1: REACH_closed m1'
        unfold exportedSrc.
        eapply REACH_cons; eassumption.*)
 
-assert (RRC: REACH_closed m1' (fun b : Values.block =>
-                         mapped (as_inj nu') b &&
-                           (locBlocksSrc nu' b
-                            || DomSrc nu' b &&
-                               (negb (locBlocksSrc nu' b) &&
-                           REACH m1' (exportedSrc nu' (ret1 :: nil)) b)))).
-  eapply REACH_closed_intersection; eassumption.
-assert (GFnu': forall b, isGlobalBlock (Genv.globalenv SrcProg) b = true ->
-               DomSrc nu' b &&
-               (negb (locBlocksSrc nu' b) && REACH m1' (exportedSrc nu' (ret1 :: nil)) b) = true).
-     intros. specialize (GF _ H).
-       assert (FSRC:= extern_incr_frgnBlocksSrc _ _ INC).
-          rewrite replace_locals_frgnBlocksSrc in FSRC.
-       rewrite FSRC in GF.
-       rewrite (frgnBlocksSrc_locBlocksSrc _ WDnu' _ GF). 
-       apply andb_true_iff; simpl.
-        split.
-          unfold DomSrc. rewrite (frgnBlocksSrc_extBlocksSrc _ WDnu' _ GF). intuition.
-          apply REACH_nil. unfold exportedSrc.
-          rewrite (frgnSrc_shared _ WDnu' _ GF). intuition.
-split.
-  unfold vis in *.
-  rewrite replace_externs_frgnBlocksSrc, replace_externs_locBlocksSrc in *.
-  econstructor; try eassumption.
-  admit.
-  rewrite replace_externs_as_inj. assumption.
-admit.
-unfold vis.
-rewrite replace_externs_locBlocksSrc, replace_externs_frgnBlocksSrc,
-        replace_externs_as_inj.
-destruct (eff_after_check2 _ _ _ _ _ MemInjNu' RValInjNu' 
-      _ (eq_refl _) _ (eq_refl _) _ (eq_refl _) WDnu' SMvalNu').
-intuition.
-Qed.
+         assert (RRC: REACH_closed m1' (fun b : Values.block =>
+                                          mapped (as_inj nu') b &&
+                                                 (locBlocksSrc nu' b
+                                                               || DomSrc nu' b &&
+                                                               (negb (locBlocksSrc nu' b) &&
+                                                                     REACH m1' (exportedSrc nu' (ret1 :: nil)) b)))).
+         eapply REACH_closed_intersection; eassumption.
+         assert (GFnu': forall b, isGlobalBlock (Genv.globalenv SrcProg) b = true ->
+                                  DomSrc nu' b &&
+                                         (negb (locBlocksSrc nu' b) && REACH m1' (exportedSrc nu' (ret1 :: nil)) b) = true).
+         intros. specialize (GF _ H).
+         assert (FSRC:= extern_incr_frgnBlocksSrc _ _ INC).
+         rewrite replace_locals_frgnBlocksSrc in FSRC.
+         rewrite FSRC in GF.
+         rewrite (frgnBlocksSrc_locBlocksSrc _ WDnu' _ GF). 
+         apply andb_true_iff; simpl.
+         split.
+         unfold DomSrc. rewrite (frgnBlocksSrc_extBlocksSrc _ WDnu' _ GF). intuition.
+         apply REACH_nil. unfold exportedSrc.
+         rewrite (frgnSrc_shared _ WDnu' _ GF). intuition.
+         split.
+         unfold vis in *.
+         rewrite replace_externs_frgnBlocksSrc, replace_externs_locBlocksSrc in *.
+         econstructor; try eassumption.
+         admit.
+         admit.
+         admit.
+         admit.
+  Qed.
 
-Hint Resolve Match_AfterExternal: trans_correct.
-eauto with trans_correct.
+  Hint Resolve Match_AfterExternal: trans_correct.
+  eauto with trans_correct.
 
-clear entry_ok.
-clear init_mem.
+  clear entry_ok.
+  clear init_mem.
 
+(*New restrict lemmas*)
+    Lemma as_inj_retrict: forall mu b1 b2 d,
+      as_inj (restrict_sm mu (vis mu)) b1 = Some (b2, d) ->
+      as_inj mu b1 = Some (b2, d).
+      intros; autorewrite with restrict in H.
+      unfold restrict in H; destruct (vis mu b1) eqn:eq; inv H; auto.
+    Qed.
 
-Ltac extend_smart:=  let x := fresh "x" in extensionality x.
+  Ltac extend_smart:=  let x := fresh "x" in extensionality x.
   Ltac rewrite_freshloc := match goal with
                              | H: (Mem.storev _ _ _ _ = Some _) |- _ => rewrite (storev_freshloc _ _ _ _ _ H)
                              | H: (Mem.free _ _ _ _ = Some _) |- _ => apply freshloc_free in H; rewrite H
@@ -1334,7 +1381,7 @@ Ltac extend_smart:=  let x := fresh "x" in extensionality x.
                            end.
   Ltac loc_alloc_solve := apply sm_locally_allocatedChar; repeat split; try extend_smart;
                           try rewrite_freshloc; intuition.
-Print sm_locally_allocated.
+  Print sm_locally_allocated.
 
   Lemma step_simulation_noeffect: forall (st1 : RTL_core) (m1 : mem) (st1' : RTL_core) (m1' : mem)
                                          (CS: corestep rtl_eff_sem ge st1 m1 st1' m1')
@@ -1366,7 +1413,7 @@ Print sm_locally_allocated.
     eapply rtl_corestep_exec_Inop. eassumption.
     exists mu.
     intuition.
-    apply intern_incr_refl.
+    (*apply intern_incr_refl.*)(* This is a Hint now*)
     apply sm_inject_separated_same_sminj.
     loc_alloc_solve.
     unfold MATCH.
@@ -1395,17 +1442,16 @@ Print sm_locally_allocated.
     exact symbols_preserved. 
     econstructor; eauto. 
     intuition.
-    apply intern_incr_refl.
+    (*apply intern_incr_refl.*)
     apply sm_inject_separated_same_sminj.
     loc_alloc_solve.
     unfold MATCH.
     intuition.
     eapply match_regular_states; eauto.
-
-
     apply match_stacks_inside_set_reg; auto.
+    SearchAbout SM_wd restrict_sm.
+    eapply restrict_sm_WD; auto.
     apply agree_set_reg; auto. 
-
 
     (* Iload *)
     exploit tr_funbody_inv; eauto. intros TR; inv TR.
@@ -1424,26 +1470,44 @@ Print sm_locally_allocated.
     eapply rtl_corestep_exec_Iload; try eassumption.
     exists mu.
     intuition.
-    apply intern_incr_refl.
+    (*apply intern_incr_refl.*)
     apply sm_inject_separated_same_sminj.
     loc_alloc_solve.
     unfold MATCH;
       intuition.
     eapply match_regular_states; eauto.
     apply match_stacks_inside_set_reg; auto.
+    eapply restrict_sm_WD; auto.
     apply agree_set_reg; auto.
     
 
     (* Istore *)
+
     exploit tr_funbody_inv; eauto. intros TR; inv TR.
+    
+    destruct H as [RC [PG [GF [SMV [WD INJ]]]]].
     exploit eval_addressing_inject.
-    About eval_addressing_inject.
-    eapply match_stacks_inside_globals; eauto.
+    eapply match_stacks_inside_globals. 
+    eassumption.
     eexact SP.
     instantiate (2 := rs##args). instantiate (1 := rs'##(sregs ctx args)). eapply agree_val_regs; eauto.
     eauto.
     fold saddr. intros [a' [P Q]].
-    exploit Mem.storev_mapped_inject; eauto. eapply agree_val_reg; eauto. 
+    Check Mem.storev_mapped_inject. 
+    Search val_inject.
+    exploit Mem.storev_mapped_inject. 
+    eexact INJ.
+    eassumption.
+    eapply val_inject_incr; try eapply Q.
+    autorewrite with restrict.
+    apply restrict_incr.
+    SearchAbout val_inject Mem.storev.
+    eapply agree_val_reg; eauto.
+    eapply agree_regs_incr.
+    eassumption.
+    autorewrite with restrict.
+    apply restrict_incr.
+    
     intros [m2' [U V]].
     assert (eval_addressing tge (Vptr sp' Int.zero) (saddr ctx addr) rs' ## (sregs ctx args) = Some a').
     rewrite <- P. apply eval_addressing_preserved. exact symbols_preserved.
@@ -1454,55 +1518,62 @@ Print sm_locally_allocated.
 
     exists mu.
     intuition.
-    apply intern_incr_refl.
+    (*apply intern_incr_refl.*)
     apply sm_inject_separated_same_sminj.
     loc_alloc_solve.
 
-
-    Focus.
     destruct a; simpl in H1; try discriminate.
     destruct a'; simpl in U; try discriminate.
+    assert (RC1': REACH_closed m1' (vis mu)).
+    eapply REACH_Store;
+    try eassumption.
+    inv Q.
+    autorewrite with restrict in H8.
+    eapply restrictD_Some.
+    eapply H8.
+    intros.
+    rewrite getBlocks_char in H5.
+    destruct H5. 
+    destruct H5.
+    Check agree_val_reg.
+    assert (val_inject (as_inj (restrict_sm mu (vis mu))) rs # src rs' # (sreg ctx src)).
+    eapply agree_val_reg; eauto.
+    rewrite H5 in H6.
+    inv H6.
+    autorewrite with restrict in H10.
+    eapply restrictD_Some.
+    eassumption.
+    simpl in H5.
+    contradiction.
+
     unfold MATCH;
-    intuition.
+      intuition.
+    (*match_states*)
     econstructor; eauto.
     eapply match_stacks_inside_store; eauto.
+    SearchAbout SM_wd restrict_sm.
+    apply restrict_sm_WD; auto.
+    autorewrite with restrict; eapply inject_restrict; try eassumption.
+    
     eapply Mem.store_valid_block_1; eauto.
     eapply range_private_invariant; eauto.
     intros; split; auto. eapply Mem.perm_store_2; eauto.
     intros; eapply Mem.perm_store_1; eauto.
     intros. eapply SSZ2. eapply Mem.perm_store_2; eauto.
     inv H2.
-    eapply REACH_Store; 
-    try eassumption.
-    assert (VINJ1: val_inject (restrict (as_inj mu) (vis mu)) (Vptr b i) (Vptr b0 i0)).
-    admit.
-    inv VINJ1.
-    apply (restrictD_Some _ _ _ _ _ H15).
-     intros b' Hb'. rewrite getBlocksD, getBlocksD_nil in Hb'.
-     destruct (rs # src); inv Hb'. 
-     rewrite orb_false_r in H10.
-       rewrite H10. simpl.
-       assert (b1=b').
-       remember (eq_block b1 b') as d.
-          destruct d; intuition.
-       subst. 
-    assert (VINJ2: val_inject (restrict (as_inj mu) (vis mu)) (Vptr b' i) (Vptr b0 i0)).
-    admit.
-       inv VINJ2. apply (restrictD_Some _ _ _ _ _ H16).
-      (* sm_valid mu m1' m2' *)
+
+    (* sm_valid mu m1' m2' *)
     split; intros. 
-      eapply storev_valid_block_1; try eassumption.
-      eapply H8; assumption.
-      eapply Mem.store_valid_block_1; try eassumption.
-      eapply H8; assumption.
+    eapply Mem.store_valid_block_1; try eassumption.
+    eapply SMV; assumption.
+    eapply Mem.store_valid_block_1; try eassumption.
+    eapply SMV; assumption.
     
-
-
-(**)
     (* Icall *)
-    Focus 1.
     exploit match_stacks_inside_globalenvs; eauto. intros [bound G].
-    exploit find_function_agree; eauto. intros [fd' [A B]].
+    exploit find_function_agree; eauto.
+    SearchAbout find_function.
+    eauto. intros [fd' [A B]].
     exploit tr_funbody_inv; eauto. intros TR. inv TR.
 
     (* not inlined *)
@@ -1514,7 +1585,7 @@ Print sm_locally_allocated.
     eapply sig_function_translated; eauto.
     exists mu.
     intuition.
-    apply intern_incr_refl.
+    (*apply intern_incr_refl.*)
     apply sm_inject_separated_same_sminj.
     loc_alloc_solve.
 
@@ -1522,6 +1593,7 @@ Print sm_locally_allocated.
     split.
     econstructor; eauto.
     eapply match_stacks_cons; eauto.
+    destruct MS0; assumption.
     eapply agree_val_regs; eauto.   
     intuition.
 
@@ -1540,15 +1612,29 @@ Print sm_locally_allocated.
 
     exists mu.
     intuition.
-    apply intern_incr_refl.
+    (*apply intern_incr_refl.*)
     apply sm_inject_separated_same_sminj.
     loc_alloc_solve.
 
     unfold MATCH;
-    intuition.
+      intuition.
     Focus 1.
     eapply match_call_regular_states; eauto. (* match_call_regular_states*)
+    assert (SL: locBlocksTgt (restrict_sm mu (vis mu)) sp' = true) by (destruct MS0; assumption).
     eapply match_stacks_inside_inlined; eauto.
+    Lemma local_of_loc_inj: forall mu b b' delta (WD: SM_wd mu) (loc: locBlocksTgt mu b' = true), as_inj  mu b = Some (b', delta) -> local_of mu b = Some (b', delta).
+      unfold as_inj. unfold join. 
+      intros.
+      destruct WD.
+      destruct (extern_of mu b) eqn:extern_mu_b; try assumption.
+      destruct p. inv H.
+      apply extern_DomRng in extern_mu_b.
+      destruct extern_mu_b as [extDom  extRng].
+      destruct (disjoint_extern_local_Tgt b'); [rewrite loc in H | rewrite extRng in H]; discriminate. 
+    Qed. (* Need to get  locBlocksTgt from MS0*)
+    apply local_of_loc_inj; auto;
+     try (apply restrict_sm_WD); auto.
+    
     red; intros. apply PRIV. inv H14. destruct H17.
     xomega.
     apply agree_val_regs_gen; auto.
@@ -1557,9 +1643,10 @@ Print sm_locally_allocated.
     (* Itailcall *)
     exploit match_stacks_inside_globalenvs; eauto. intros [bound G].
     exploit find_function_agree; eauto. intros [fd' [A B]].
-    assert (PRIV': range_private (as_inj mu) m1' m2 sp' (dstk ctx) f'.(fn_stacksize)).
-    eapply range_private_free_left; eauto. inv FB. rewrite <- H5. auto. 
-    exploit tr_funbody_inv; eauto. 
+    assert (PRIV': range_private (as_inj (restrict_sm mu (vis mu))) m1' m2 sp' (dstk ctx) f'.(fn_stacksize)).
+    eapply range_private_free_left; eauto. 
+    inv FB. rewrite <- H5. auto.
+    exploit tr_funbody_inv; eauto.
     intros TR. 
     inv TR.
 
@@ -1581,16 +1668,34 @@ Print sm_locally_allocated.
     eapply sig_function_translated; eauto.
     exists mu.
     intuition.
-    apply intern_incr_refl.
+    (*apply intern_incr_refl.*)
     apply sm_inject_separated_same_sminj.
     loc_alloc_solve.
-     
     
+    assert (Mem.inject (as_inj mu) m1' m2').
+    eapply Mem.free_right_inject. eapply Mem.free_left_inject. eapply H12.
+    eassumption.
+    eassumption.
+
+    intros. rewrite DSTK in PRIV'. exploit (PRIV' (ofs + delta)). omega. intros [P Q]. 
+    eelim Q.
+    autorewrite with restrict.
+    eapply restrictI_Some.
+    eapply H11.
+    rewrite restrict_sm_locBlocksTgt in SL.
+    erewrite <- (as_inj_locBlocks _ b1 sp') in SL; try eassumption.
+    unfold vis.
+    rewrite SL.
+    eapply orb_true_l.
+    replace (ofs + delta - delta) with ofs by omega.
+    apply Mem.perm_max with k. apply Mem.perm_implies with p; auto with mem.
+
     unfold MATCH.
     intuition.
     econstructor; eauto.
     eapply match_stacks_bound with (bound := sp'). 
     eapply match_stacks_invariant; eauto.
+    apply restrict_sm_WD; auto.
     intros. eapply Mem.perm_free_3; eauto. 
     intros. eapply Mem.perm_free_1; eauto. 
     intros. eapply Mem.perm_free_3; eauto.
@@ -1602,18 +1707,26 @@ Print sm_locally_allocated.
     eelim Q; eauto. replace (ofs + delta - delta) with ofs by omega. 
     apply Mem.perm_max with k. apply Mem.perm_implies with p; auto with mem.
     eapply REACH_closed_free; eauto.
-      (* sm_valid mu m1' m2' *)
+    (* sm_valid mu m1' m2' *)
     split; intros. 
-      eapply Mem.valid_block_free_1; try eassumption.
-      eapply H7; assumption.
-      eapply Mem.valid_block_free_1; try eassumption.
-      eapply H7; assumption.
-      (*  Mem.inject (as_inj mu) m1' m2' *)
-      eapply Mem.free_right_inject; eauto. eapply Mem.free_left_inject; eauto.
-      (* show that no valid location points into the stack block being freed *)
-      intros. rewrite DSTK in PRIV'. exploit (PRIV' (ofs + delta)). omega. intros [P Q]. 
-      eelim Q; eauto. replace (ofs + delta - delta) with ofs by omega. 
-      apply Mem.perm_max with k. apply Mem.perm_implies with p; auto with mem.
+    eapply Mem.valid_block_free_1; try eassumption.
+    eapply H7; assumption.
+    eapply Mem.valid_block_free_1; try eassumption.
+    eapply H7; assumption.
+    (*  Mem.inject (as_inj mu) m1' m2' *)(* Got it for free*)
+    (* eapply Mem.free_right_inject; eauto. eapply Mem.free_left_inject; eauto.*)
+    (* show that no valid location points into the stack block being freed *)
+    (*The following isnot needed*)
+    (*intros. rewrite DSTK in PRIV'. exploit (PRIV' (ofs + delta)). omega. intros [P Q]. 
+    eelim Q.
+    assert (HH: vis mu b1 = true).
+    admit.
+    instantiate (2:= b1).
+    autorewrite with restrict. 
+    unfold restrict. erewrite HH; simpl; eauto.
+    replace (ofs + delta - delta) with (ofs) by omega. 
+(*    replace (ofs + delta - dstk ctx) with ofs by omega. *)
+    apply Mem.perm_max with k. apply Mem.perm_implies with p; auto with mem.*)
 
     (* turned into a call *)
     eexists. eexists. split; simpl.
@@ -1623,7 +1736,7 @@ Print sm_locally_allocated.
     
     exists mu.
     intuition.
-    apply intern_incr_refl.
+    (*apply intern_incr_refl.*)
     apply sm_inject_separated_same_sminj.
     loc_alloc_solve.
 
@@ -1632,18 +1745,21 @@ Print sm_locally_allocated.
     econstructor; eauto.
     eapply match_stacks_untailcall; eauto.
     eapply match_stacks_inside_invariant; eauto. 
+    apply restrict_sm_WD; auto.
     intros. eapply Mem.perm_free_3; eauto.
+    destruct MS0; assumption.
+   
     eapply agree_val_regs; eauto.
     eapply Mem.free_left_inject; eauto.
     eapply REACH_closed_free; eauto.
     
     (*  sm_valid mu m1' m2 *)
     split; intros. 
-      eapply Mem.valid_block_free_1; try eassumption.
-      eapply H7; assumption.
-      eapply H7; assumption.
-      (*  Mem.inject (as_inj mu) m1' m2' *)
-      eapply Mem.free_left_inject; eauto.
+    eapply Mem.valid_block_free_1; try eassumption.
+    eapply H7; assumption.
+    eapply H7; assumption.
+    (*  Mem.inject (as_inj mu) m1' m2' *)
+    eapply Mem.free_left_inject; eauto.
 
     (* inlined *)
     assert (fd = Internal f0).
@@ -1658,15 +1774,16 @@ Print sm_locally_allocated.
 
     exists mu.
     intuition.
-    apply intern_incr_refl.
+    (*apply intern_incr_refl.*)
     apply sm_inject_separated_same_sminj.
     loc_alloc_solve.
 
     unfold MATCH;
-    intuition.
+      intuition.
     econstructor; eauto.
     eapply match_stacks_inside_inlined_tailcall; eauto.
     eapply match_stacks_inside_invariant; eauto.
+    apply restrict_sm_WD; auto.
     intros. eapply Mem.perm_free_3; eauto.
     apply agree_val_regs_gen; auto.
     eapply Mem.free_left_inject; eauto.
@@ -1676,11 +1793,11 @@ Print sm_locally_allocated.
     eapply REACH_closed_free; eauto.
     (* sm_valid mu m1' m2 *)
     split; intros.
-      eapply Mem.valid_block_free_1; try eassumption.
-      eapply H11; assumption.
-      eapply H11; assumption.
-      (*  Mem.inject (as_inj mu) m1' m2' *)
-      eapply Mem.free_left_inject; eauto.
+    eapply Mem.valid_block_free_1; try eassumption.
+    eapply H11; assumption.
+    eapply H11; assumption.
+    (*  Mem.inject (as_inj mu) m1' m2' *)
+    eapply Mem.free_left_inject; eauto.
 
 
     (* Icond *)
@@ -1696,7 +1813,7 @@ Print sm_locally_allocated.
     eapply rtl_corestep_exec_Icond; eauto.
 
     exists mu. intuition.
-    apply intern_incr_refl.
+    (*apply intern_incr_refl.*)
     apply sm_inject_separated_same_sminj.
     loc_alloc_solve.
 
@@ -1708,7 +1825,7 @@ Print sm_locally_allocated.
 
     (* jumptable *)
     exploit tr_funbody_inv; eauto. intros TR; inv TR.
-    assert (val_inject (as_inj mu) rs#arg rs'#(sreg ctx arg)). eapply agree_val_reg; eauto.
+    assert (H3: val_inject (as_inj (restrict_sm mu (vis mu))) rs#arg rs'#(sreg ctx arg)). eapply agree_val_reg; eauto.
     rewrite H1 in H3; inv H3.
     
     eexists. eexists.
@@ -1718,13 +1835,14 @@ Print sm_locally_allocated.
     rewrite list_nth_z_map. rewrite H2. simpl; reflexivity. 
     
     exists mu. intuition.
-    apply intern_incr_refl.
+    (*apply intern_incr_refl.*)
     apply sm_inject_separated_same_sminj.
     loc_alloc_solve.
 
     unfold MATCH.
     intuition.
     econstructor; eauto.
+
 
     (* return *)
     exploit tr_funbody_inv; eauto. intros TR; inv TR.
@@ -1747,15 +1865,16 @@ Print sm_locally_allocated.
     
     exists mu.
     intuition.
-    apply intern_incr_refl.
+    (* apply intern_incr_refl. *)
     apply sm_inject_separated_same_sminj.
     loc_alloc_solve.
 
     unfold MATCH;
-    intuition.
+      intuition.
     econstructor; eauto.
     eapply match_stacks_bound with (bound := sp'). 
     eapply match_stacks_invariant; eauto.
+    apply restrict_sm_WD; auto.
     intros. eapply Mem.perm_free_3; eauto. 
     intros. eapply Mem.perm_free_1; eauto. 
     intros. eapply Mem.perm_free_3; eauto.
@@ -1765,7 +1884,7 @@ Print sm_locally_allocated.
     eapply Mem.free_right_inject; eauto. eapply Mem.free_left_inject; eauto.
     (* show that no valid location points into the stack block being freed *)
     intros. inversion FB; subst.
-    assert (PRIV': range_private (as_inj mu) m1' m2 sp' (dstk ctx) f'.(fn_stacksize)).
+    assert (PRIV': range_private (as_inj (restrict_sm mu (vis mu))) m1' m2 sp' (dstk ctx) f'.(fn_stacksize)).
     rewrite H16 in PRIV. eapply range_private_free_left; eauto. 
     rewrite DSTK in PRIV'. exploit (PRIV' (ofs + delta)). omega. intros [A B]. 
     eelim B; eauto. replace (ofs + delta - delta) with ofs by omega. 
@@ -1775,21 +1894,29 @@ Print sm_locally_allocated.
 
     (*  sm_valid mu m1' m2 *)
     split; intros.
-      eapply Mem.valid_block_free_1; try eassumption.
-      eapply H8; assumption.
-      eapply Mem.valid_block_free_1; try eassumption.
-      eapply H8; assumption.
-      (*  Mem.inject (as_inj mu) m1' m2' *)
- eapply Mem.free_right_inject; eauto. eapply Mem.free_left_inject; eauto.
+    eapply Mem.valid_block_free_1; try eassumption.
+    eapply H8; assumption.
+    eapply Mem.valid_block_free_1; try eassumption.
+    eapply H8; assumption.
+    (*  Mem.inject (as_inj mu) m1' m2' *)
+    eapply Mem.free_right_inject; eauto. eapply Mem.free_left_inject; eauto.
     (* show that no valid location points into the stack block being freed *)
     intros. inversion FB; subst.
-    assert (PRIV': range_private (as_inj mu) m1' m2 sp' (dstk ctx) f'.(fn_stacksize)).
+    assert (PRIV': range_private (as_inj (restrict_sm mu (vis mu))) m1' m2 sp' (dstk ctx) f'.(fn_stacksize)).
     rewrite H16 in PRIV. eapply range_private_free_left; eauto. 
     rewrite DSTK in PRIV'. exploit (PRIV' (ofs + delta)). omega. intros [A B]. 
-    eelim B; eauto. replace (ofs + delta - delta) with ofs by omega. 
+    eelim B. 
+    autorewrite with restrict.
+    eapply restrictI_Some.
+    apply H10.
+    rewrite restrict_sm_locBlocksTgt in SL.
+    erewrite <- (as_inj_locBlocks _ b1 sp') in SL; try eassumption.
+    unfold vis.
+    rewrite SL.
+    eapply orb_true_l.
+    replace (ofs + delta - delta) with ofs by omega.
     apply Mem.perm_max with k. apply Mem.perm_implies with p; auto with mem.
-
-
+    
     (* inlined *)
     eexists. eexists.             
     split; simpl.
@@ -1799,29 +1926,32 @@ Print sm_locally_allocated.
 
     exists mu.
     intuition.
-    apply intern_incr_refl.
+    (*apply intern_incr_refl.*)
+
     apply sm_inject_separated_same_sminj.
     loc_alloc_solve. 
     
     unfold MATCH;
-    intuition.
+      intuition.
     econstructor; eauto.
     
     
-  eapply match_stacks_inside_invariant; eauto. 
+    eapply match_stacks_inside_invariant; eauto. 
+    apply restrict_sm_WD; auto.
     intros. eapply Mem.perm_free_3; eauto.
-  destruct or; simpl. apply agree_val_reg; auto. auto.
-  eapply Mem.free_left_inject; eauto.
-  inv FB. subst.  rewrite H13 in PRIV. eapply range_private_free_left; eauto.
-  
+    destruct or; simpl. apply agree_val_reg; auto. auto.
+    eapply Mem.free_left_inject; eauto.
+    inv FB. subst.  rewrite H13 in PRIV. eapply range_private_free_left; eauto.
+    
     eapply REACH_closed_free; eauto.
     (*sm_valid*)
     split; intros.
-      eapply Mem.valid_block_free_1; try eassumption.
-      eapply H8; assumption.
-      eapply H8; assumption.
-      (*  Mem.inject (as_inj mu) m1' m2 *)
-      eapply Mem.free_left_inject; eauto.
+    eapply Mem.valid_block_free_1; try eassumption.
+    eapply H8; assumption.
+    eapply H8; assumption.
+    (*  Mem.inject (as_inj mu) m1' m2 *)
+    eapply Mem.free_left_inject; eauto.
+    Print corestep.
 
     (* internal function, not inlined *)
     assert (A: exists f', tr_function fenv f f' /\ fd' = Internal f'). 
@@ -1829,7 +1959,7 @@ Print sm_locally_allocated.
     destruct A as [f' [TR EQ]]. inversion TR; subst.
     repeat open_Hyp.
     exploit alloc_parallel_intern; 
-    eauto. apply Zle_refl. 
+      eauto. apply Zle_refl. 
     instantiate (1 := fn_stacksize f'). inv H1. xomega.
     intros [mu' [m2' [sp' [A [B [C [D E]]]]]]].
     
@@ -1845,97 +1975,350 @@ Print sm_locally_allocated.
     unfold MATCH; intuition.
     rewrite H6.
     rewrite <- H5.
-    eapply match_regular_states.
+    
+    eapply match_regular_states; eauto.
+    assert (SP: sp' = Mem.nextblock m2) by (eapply Mem.alloc_result; eauto).
     apply match_stacks_inside_base.
-  assert (SP: sp' = Mem.nextblock m2) by (eapply Mem.alloc_result; eauto).
-  rewrite <- SP in MS0. 
-  eapply (match_stacks_invariant mu); eauto.
-    eapply intern_incr_as_inj; eauto.
-    intros. destruct (eq_block b1 stk). 
-    subst b1. rewrite D in H20; inv H20. subst b2. eelim Plt_strict; eauto.  
-    rewrite H14 in H20; auto. 
+    rewrite <- SP in MS0. 
+    eapply (match_stacks_invariant (restrict_sm mu (vis mu))); eauto.
+    eapply restrict_sm_intern_incr; auto.
+    eapply restrict_sm_WD; auto.
+    
+    intros. 
+    destruct (eq_block b1 stk). 
+    subst b1.
+    apply as_inj_retrict  in H20; rewrite D in H20; inv H20. subst b2. eelim Plt_strict; eauto.
+    rewrite <- H20.
+    autorewrite with restrict.
+    unfold restrict.
+    rewrite H14; auto.
+    assert (vis mu' b1 = true ) by admit.
+    erewrite (intern_incr_vis_inv mu mu'); auto.
+    rewrite H22; auto.
+    rewrite <- H14; auto.
+    apply as_inj_retrict in H20; eassumption.
+    
     intros. exploit Mem.perm_alloc_inv. eexact H0. eauto. 
     destruct (eq_block b1 stk); intros; auto. 
-    subst b1. rewrite D in H20; inv H20. subst b2. eelim Plt_strict; eauto.  
+    subst b1. apply as_inj_retrict in H20.
+    rewrite D in H20; inv H20. subst b2. eelim Plt_strict; eauto.  
+
     intros. eapply Mem.perm_alloc_1; eauto. 
     intros. exploit Mem.perm_alloc_inv. eexact A. eauto. 
     rewrite dec_eq_false; auto.
-  auto. auto. auto. 
-  rewrite H5. apply agree_regs_init_regs.
-  eapply val_list_inject_incr.
-  Lemma inject_incr_structure: forall mu mu' (II: intern_incr mu mu'), inject_incr (as_inj mu) (as_inj mu').
-  Admitted.
-  eapply inject_incr_structure; eauto.
-  eauto.
-  auto. inv H1; auto. congruence. auto.
-  eapply Mem.valid_new_block; eauto.
-  red; intros. split.
-  eapply Mem.perm_alloc_2; eauto. inv H1; xomega.
-  intros; red; intros. exploit Mem.perm_alloc_inv. eexact H0. eauto.
-  destruct (eq_block b stk); intros. 
-  subst. rewrite D in H21; inv H21. inv H1; xomega.
-  rewrite H14 in H21; auto. eelim Mem.fresh_block_alloc. eexact A. eapply Mem.mi_mappedblocks; eauto.
-  auto.
-  intros. exploit Mem.perm_alloc_inv; eauto. rewrite dec_eq_true. omega.
 
-  (* meminj_preserves_globals ge (as_inj mu') 
-  unfold meminj_preserves_globals in H9.
-   destruct H9 as [A' [B' C']].
-   unfold meminj_preserves_globals; intros. 
-   repeat split; intros.
-   destruct (eq_block b stk); intros. 
-   subst b. 
-   rewrite D.*)
-   
-  admit.
-  admit.
+    (*This should be a lemma! *)
+    Lemma alloc_local_restrict: forall mu mu' m1 m2 m1' m2' sp' f' (A : Mem.alloc m2 0 (fn_stacksize f') = (m2', sp')) (H15 : sm_locally_allocated mu mu' m1 m2 m1' m2') (SP: sp' = Mem.nextblock m2), locBlocksTgt (restrict_sm mu' (vis mu')) sp' = true.
+      intros.
+      unfold sm_locally_allocated in H15.
+    destruct mu.
+    destruct mu'; simpl in *.
+    intuition.
+    rewrite H1.
+    assert (fl: freshloc m2 m2' sp' = true).
+    unfold freshloc.
+    assert (vb: ~ Mem.valid_block m2 sp').
+    unfold Mem.valid_block.
+    subst sp'.
+    xomega.
+    assert (vb': Mem.valid_block m2' sp').
+    unfold Mem.valid_block.
+    (*erewrite (Mem.nextblock_alloc m2 _ _ m2' sp').*)
+    rewrite (Mem.nextblock_alloc m2 0 (fn_stacksize f') m2' sp').
+    subst sp'.
+    xomega.
+    subst sp'.
+    exact A.
+    destruct (valid_block_dec m2' sp'); destruct (valid_block_dec m2 sp'); intuition.
+    rewrite fl; apply orb_true_r.
+    Qed.
+    (*End of theorem.*)
+    eapply alloc_local_restrict; eauto.
+
+    auto. auto. auto.
+    rewrite H5. apply agree_regs_init_regs.
+    Check val_list_inject_incr.
+    eapply val_list_inject_incr.
+    autorewrite with restrict.
+    eapply intern_incr_restrict; try (apply C); auto.
+    autorewrite with restrict in VINJ; auto.
+    inv H1; auto. 
+    Print Mem.alloc.
+    autorewrite with restrict.
+    unfold restrict.
+    rewrite D.
+    unfold vis.
 
 
-    (* internal function, inlined *)
-    inversion FB; subst.
-    exploit Mem.alloc_left_mapped_inject. 
-    eauto.
-    eauto.
-    (* sp' is valid *)
-    instantiate (1 := sp'). auto.
-    (* offset is representable *)
-    instantiate (1 := dstk ctx). generalize (Zmax2 (fn_stacksize f) 0). omega.
-    (* size of target block is representable *)
-    intros. right. exploit SSZ2; eauto with mem. inv FB; omega.
-    (* we have full permissions on sp' at and above dstk ctx *)
-    intros. apply Mem.perm_cur. apply Mem.perm_implies with Freeable; auto with mem.
-    eapply range_private_perms; eauto. xomega.
-    (* offset is aligned *)
-    replace (fn_stacksize f - 0) with (fn_stacksize f) by omega.
-    inv FB. apply min_alignment_sound; auto.
-    (* nobody maps to (sp, dstk ctx...) *)
-    intros. exploit (PRIV (ofs + delta')); eauto. xomega.
-    intros [A B]. eelim B; eauto.
-    replace (ofs + delta' - delta') with ofs by omega.
-    apply Mem.perm_max with k. apply Mem.perm_implies with p; auto with mem.
-    intros [F' [A [B [C D]]]].
-    exploit tr_moves_init_regs; eauto. intros [rs'' [P [Q R]]].
-    eexists. eexists.
-    split; simpl. 
-    left.
-    eapply core_semantics_lemmas.corestep_plus_one. eapply rtl_corestep_exec_Inop; eauto. 
-    Print star.
-    (* eexact P. traceEq.
-  eapply match_regular_states.
-  econstructor.
-  eapply match_stacks_inside_alloc_left; eauto.
-  eapply match_stacks_inside_invariant; eauto.
-  omega.
-  auto.
-  apply agree_regs_incr with F; auto.
-  auto. auto. auto.
-  rewrite H2. eapply range_private_alloc_left; eauto.
-  auto. auto.*)
-    clear P. admit.
-    
+    (*This should be a lemma*)
+    assert (locBlocksSrc mu' stk = true).
+    rewrite (Mem.alloc_result _ _ _ _ stk H0).
+    rewrite (Mem.alloc_result _ _ _ _ stk H0) in H0.
+    unfold sm_locally_allocated in H15.
+    destruct mu; destruct mu'; simpl in *.
+    intuition.
+    rewrite H20.
+    assert (fl: freshloc m1 m1' (Mem.nextblock m1) = true).
+    unfold freshloc.
+    assert (vb: ~ Mem.valid_block m1 (Mem.nextblock m1)).
+    unfold Mem.valid_block.
+    xomega.
+    assert (vb': Mem.valid_block m1' (Mem.nextblock m1)).
+    unfold Mem.valid_block.
+    rewrite (Mem.nextblock_alloc m1 0 (fn_stacksize f) m1' (Mem.nextblock m1)).
+    xomega.
+    auto.
+    destruct (valid_block_dec m1' (Mem.nextblock m1)); destruct (valid_block_dec m1 (Mem.nextblock m1)); intuition.
+    rewrite fl; apply orb_true_r.
 
-    (* external function *)
-    (*  exploit match_stacks_globalenvs; eauto. intros [bound MG].
+    (*End of Lemma *)
+
+
+    rewrite H20. rewrite orb_true_l.
+    rewrite H2; auto.
+
+    autorewrite with restrict.
+    apply inject_restrict; auto.
+
+    eapply Mem.valid_new_block; eauto.
+    red; intros. split.
+    eapply Mem.perm_alloc_2; eauto. inv H1; xomega.
+    intros; red; intros. exploit Mem.perm_alloc_inv. eexact H0. eauto.
+    destruct (eq_block b stk); intros; apply as_inj_retrict in H21. 
+    subst. 
+    rewrite D in H21; inv H21. inv H1; xomega.
+    rewrite H14 in H21; auto. eelim Mem.fresh_block_alloc. eexact A.
+    eapply Mem.mi_mappedblocks.
+    apply H13.
+    apply H21.
+
+
+    intros.
+    exploit Mem.perm_alloc_3; eauto.
+    xomega.
+
+    apply (meminj_preserves_incr_sep ge (as_inj mu) H9 m1 m2); eauto.
+    apply intern_incr_as_inj; auto.
+    apply sm_inject_separated_mem; auto.
+
+    Check intern_incr_meminj_preserves_globals_as_inj.
+    eapply intern_incr_meminj_preserves_globals_as_inj in H17.
+    destruct H17 as [H00 H01]; apply H01; auto.
+    eexact H20.
+    exact H12.
+    split; eauto.
+    assumption.
+
+(* internal function, inlined *)
+inversion FB; subst.
+repeat open_Hyp.
+exploit alloc_left_mapped_sm_inject; try eassumption.
+(* sp' is local *)
+destruct MS0; unfold locBlocksTgt in SL; unfold restrict_sm in SL; destruct mu; simpl in *; assumption.
+(* offset is representable *)
+instantiate (1 := dstk ctx). generalize (Zmax2 (fn_stacksize f) 0). omega.
+(* size of target block is representable *)
+intros. right. exploit SSZ2; eauto with mem. inv FB; omega.
+(* we have full permissions on sp' at and above dstk ctx *)
+intros. apply Mem.perm_cur. apply Mem.perm_implies with Freeable; auto with mem.
+eapply range_private_perms; eauto. xomega.
+(* offset is aligned *)
+replace (fn_stacksize f - 0) with (fn_stacksize f) by omega.
+inv FB. apply min_alignment_sound; auto.
+(* nobody maps to (sp, dstk ctx...) *)
+intros. exploit (PRIV (ofs + delta')); eauto. xomega.
+intros [A B]. apply (B b delta'); eauto.
+assert (SL': locBlocksTgt mu sp' = true).
+destruct MS0; unfold locBlocksTgt in SL; unfold restrict_sm in SL; destruct mu; simpl in *; assumption.
+rewrite <- (as_inj_locBlocks mu b sp' delta') in SL'; auto.
+autorewrite with restrict.
+unfold restrict; unfold vis.
+rewrite SL'.
+rewrite orb_true_l; simpl; assumption.
+replace (ofs + delta' - delta') with ofs by omega.
+apply Mem.perm_max with k. apply Mem.perm_implies with p; auto with mem.
+intros [mu' [A [B [C D]]]].
+(*
+tr_moves_init_regs
+     : forall (F : meminj) (stk : list stackframe) 
+         (f : function) (sp : val) (m : mem) (ctx1 ctx2 : context),
+       context_below ctx1 ctx2 ->
+       forall (rdsts rsrcs : list reg) (vl : list val) 
+         (pc1 pc2 : node) (rs1 : regset),
+       tr_moves (fn_code f) pc1 (sregs ctx1 rsrcs) (sregs ctx2 rdsts) pc2 ->
+       (forall r : reg, In r rdsts -> Ple r (mreg ctx2)) ->
+       list_forall2 (val_reg_charact F ctx1 rs1) vl rsrcs ->
+       exists rs2 : regset,
+         star step tge (State stk f sp pc1 rs1 m) E0
+           (State stk f sp pc2 rs2 m) /\
+         agree_regs F ctx2 (init_regs vl rdsts) rs2 /\
+         (forall r : positive, Plt r (dreg ctx2) -> rs2 # r = rs1 # r)
+*)
+exploit tr_moves_init_regs; eauto. intros [rs'' [P [Q R]]].
+eexists. eexists.
+split; simpl. 
+left.
+eapply core_semantics_lemmas.corestep_plus_star_trans.
+(* eapply core_semantics_lemmas.corestep_plus_one. *)
+eapply core_semantics_lemmas.corestep_plus_one.
+eapply rtl_corestep_exec_Inop; eauto. 
+induction P.
+apply core_semantics_lemmas.corestep_star_zero.
+eapply core_semantics_lemmas.corestep_star_trans.
+apply core_semantics_lemmas.corestep_star_one.
+Focus 2.
+apply IHP.
+Search core_semantics_lemmas.corestep_star.
+
+
+exists mu'; intuition.
+
+Lemma sm_inject_separated_impication: forall mu mu' m1 m2 m1' m2' stk sp' delta (laloc: sm_locally_allocated mu mu' m1 m2 m1' m2')(C: as_inj mu' stk = Some (sp', delta))(H14: forall b : block, (b = stk -> False) -> as_inj mu' b = as_inj mu b)(WD: SM_wd mu) (WD': SM_wd mu'), sm_inject_separated mu mu' m1 m2.
+Admitted.
+
+eapply sm_inject_separated_impication; eauto.
+
+unfold MATCH. 
+split.
+inv P.
+Focus 2. 
+Print star.
+
+
+star step tge (State ?176062 f' ?176063 pc1' rs' ?176064) E0
+        (State ?176062 f' ?176063 (spc ctx (fn_entrypoint f)) rs'' ?176064).
+
+
+eapply match_regular_states.
+Print match_stacks_inside.
+eapply match_stacks_inside_alloc_left. 
+apply restrict_sm_WD.
+apply H12.
+intros b HH; apply HH.
+apply MS0.
+apply restrict_sm_WD; intros; assumption.
+eassumption.
+eapply restrict_sm_intern_incr; try assumption.
+autorewrite with restrict.
+unfold restrict; unfold vis.
+erewrite as_inj_locBlocks; eauto.
+
+assert (loc_sp: locBlocksTgt mu sp' = true).
+destruct MS0; unfold restrict_sm in SL; destruct mu; simpl in *; eassumption.
+
+unfold sm_locally_allocated in H17.
+destruct mu; destruct mu'; simpl in H17; simpl in *.
+repeat open_Hyp;
+subst locBlocksTgt0.
+rewrite loc_sp.
+repeat rewrite orb_true_l.
+eassumption.
+
+intros.
+autorewrite with restrict.
+unfold restrict; unfold vis.
+inv B.
+repeat open_Hyp.
+rewrite H26.
+rewrite H14; auto.
+destruct (locBlocksSrc mu b1) eqn: lbl_eq.
+rewrite H22; auto.
+assert (HH: freshloc m1 m1' b1 = false).
+SearchAbout freshloc Mem.alloc.
+apply freshloc_alloc in H0; rewrite H0. 
+destruct eq_block; intuition.
+
+unfold sm_locally_allocated in H17; destruct mu; destruct mu'; simpl in *.
+repeat open_Hyp.
+subst locBlocksSrc0.
+rewrite lbl_eq. 
+rewrite HH.
+simpl.
+auto.
+
+xomega.
+
+auto.
+
+auto.
+
+eapply agree_regs_incr; eauto.
+
+autorewrite with restrict.
+apply intern_incr_restrict; auto.
+
+
+assert (SL: locBlocksTgt (restrict_sm mu (vis mu)) sp' = true ).
+inv MS0; assumption.
+assert (SL': locBlocksTgt mu sp' = true ).
+unfold restrict_sm in SL. destruct mu; simpl in *; assumption.
+assert (SL'': locBlocksTgt mu' sp' = true ).
+unfold sm_locally_allocated in H17.
+
+destruct mu; destruct mu'; repeat open_Hyp; simpl in *; subst locBlocksTgt0;
+rewrite SL'; rewrite orb_true_l; auto.
+
+autorewrite with restrict.
+unfold restrict; unfold vis.
+erewrite as_inj_locBlocks; eauto. rewrite SL''; rewrite orb_true_l; auto.
+
+autorewrite with restrict.
+apply inject_restrict; auto.
+
+auto.
+
+Check range_private_alloc_left. rewrite H3.
+eapply range_private_alloc_left; eauto.
+
+assert (SL: locBlocksTgt (restrict_sm mu (vis mu)) sp' = true ).
+inv MS0; assumption.
+assert (SL': locBlocksTgt mu sp' = true ).
+unfold restrict_sm in SL. destruct mu; simpl in *; assumption.
+assert (SL'': locBlocksTgt mu' sp' = true ).
+unfold sm_locally_allocated in H17.
+destruct mu; destruct mu'; repeat open_Hyp; simpl in *; subst locBlocksTgt0;
+rewrite SL'; rewrite orb_true_l; auto.
+
+autorewrite with restrict.
+erewrite <- as_inj_locBlocks in SL''; eauto.
+
+unfold restrict; unfold vis; rewrite SL''. rewrite orb_true_l; simpl; auto.
+
+intros.
+autorewrite with restrict.
+unfold restrict; unfold vis.
+inv B.
+repeat open_Hyp.
+rewrite H26.
+rewrite H14; auto.
+destruct (locBlocksSrc mu b) eqn: lbl_eq.
+rewrite H22; auto.
+assert (HH: freshloc m1 m1' b = false).
+SearchAbout freshloc Mem.alloc.
+apply freshloc_alloc in H0; rewrite H0. 
+destruct eq_block; intuition.
+
+
+unfold sm_locally_allocated in H17; destruct mu; destruct mu'; simpl in *.
+repeat open_Hyp.
+subst locBlocksSrc0.
+rewrite lbl_eq. 
+rewrite HH.
+simpl.
+auto.
+
+xomega.
+
+auto.
+
+Print star.
+
+econstructor.
+
+
+
+(* external function *)
+(*  exploit match_stacks_globalenvs; eauto. intros [bound MG].
   (*exploit external_call_mem_inject; eauto.
     eapply match_globalenvs_preserves_globals; eauto.
     Check external_call.
@@ -1955,81 +2338,81 @@ Print sm_locally_allocated.
     eapply external_call_nextblock; eauto. 
     auto. auto.*)
 
-    (* return fron noninlined function *)
-    inv MS0.
-    (* normal case *)
-    eexists. eexists.
-    split; simpl.
-    left.
-    eapply core_semantics_lemmas.corestep_plus_one. eapply rtl_corestep_exec_return.
-    
-    exists mu. intuition.
-    apply intern_incr_refl.
-    apply sm_inject_separated_same_sminj.
-    loc_alloc_solve.
+(* return fron noninlined function *)
+inv MS0.
+(* normal case *)
+eexists. eexists.
+split; simpl.
+left.
+eapply core_semantics_lemmas.corestep_plus_one. eapply rtl_corestep_exec_return.
 
-    unfold MATCH; intuition.
-    econstructor; eauto. 
-    apply match_stacks_inside_set_reg; auto. 
-    apply agree_set_reg; auto.
-    
-    (* untailcall case *)
-    inv MS; try congruence.
-    rewrite RET in RET0; inv RET0.
-    (*
+exists mu. intuition.
+apply intern_incr_refl.
+apply sm_inject_separated_same_sminj.
+loc_alloc_solve.
+
+unfold MATCH; intuition.
+econstructor; eauto. 
+apply match_stacks_inside_set_reg; auto. 
+apply agree_set_reg; auto.
+
+(* untailcall case *)
+inv MS; try congruence.
+rewrite RET in RET0; inv RET0.
+(*
   assert (rpc = pc). unfold spc in H0; unfold node in *; xomega.
   assert (res0 = res). unfold sreg in H1; unfold reg in *; xomega.
   subst rpc res0.
-     *)
-    eexists. eexists.     
-    split; simpl.
-    left.
-    eapply core_semantics_lemmas.corestep_plus_one. eapply rtl_corestep_exec_return.
-    exists mu. intuition.
-    apply intern_incr_refl.
-    apply sm_inject_separated_same_sminj.
-    loc_alloc_solve.
+ *)
+eexists. eexists.     
+split; simpl.
+left.
+eapply core_semantics_lemmas.corestep_plus_one. eapply rtl_corestep_exec_return.
+exists mu. intuition.
+apply intern_incr_refl.
+apply sm_inject_separated_same_sminj.
+loc_alloc_solve.
 
-    unfold MATCH. intuition.
-    eapply match_regular_states. 
-    eapply match_stacks_inside_set_reg; eauto.
-    auto. 
-    apply agree_set_reg; auto.
-    auto. auto. auto.
-    red; intros. destruct (zlt ofs (dstk ctx)). apply PAD; omega. apply PRIV; omega.
-    auto. auto. 
-    
-    (* return from inlined function *)
-    inv MS0; try congruence. rewrite RET0 in RET; inv RET. 
-    unfold inline_return in AT. 
-    assert (PRIV': range_private (as_inj mu) m1' m2 sp' (dstk ctx' + mstk ctx') f'.(fn_stacksize)).
-    red; intros. destruct (zlt ofs (dstk ctx)). apply PAD. omega. apply PRIV. omega.
-    (* with a result *)
-    destruct or.
-    eexists. eexists.
-    split; simpl.
-    left. 
-    eapply core_semantics_lemmas.corestep_plus_one.
-    eapply rtl_corestep_exec_Iop; eauto. simpl. reflexivity.
-    
-    exists mu. intuition.
-    apply intern_incr_refl.
-    apply sm_inject_separated_same_sminj.
-    loc_alloc_solve.
+unfold MATCH. intuition.
+eapply match_regular_states. 
+eapply match_stacks_inside_set_reg; eauto.
+auto. 
+apply agree_set_reg; auto.
+auto. auto. auto.
+red; intros. destruct (zlt ofs (dstk ctx)). apply PAD; omega. apply PRIV; omega.
+auto. auto. 
 
-    unfold MATCH; intuition.
-    econstructor; eauto. apply match_stacks_inside_set_reg; auto. apply agree_set_reg; auto.
-    (* without a result *)
-    eexists. eexists.
-    split; simpl. left.  
-    eapply core_semantics_lemmas.corestep_plus_one. eapply rtl_corestep_exec_Inop; eauto.
-    exists mu. intuition.
-    apply intern_incr_refl.
-    apply sm_inject_separated_same_sminj.
-    apply sm_locally_allocatedChar.
-    repeat split; extensionality b0;
-    rewrite freshloc_irrefl;
-    intuition.
-    unfold MATCH; intuition.
-    econstructor; eauto. subst vres. apply agree_set_reg_undef'; auto.
-  Qed.
+(* return from inlined function *)
+inv MS0; try congruence. rewrite RET0 in RET; inv RET. 
+unfold inline_return in AT. 
+assert (PRIV': range_private (as_inj mu) m1' m2 sp' (dstk ctx' + mstk ctx') f'.(fn_stacksize)).
+red; intros. destruct (zlt ofs (dstk ctx)). apply PAD. omega. apply PRIV. omega.
+(* with a result *)
+destruct or.
+eexists. eexists.
+split; simpl.
+left. 
+eapply core_semantics_lemmas.corestep_plus_one.
+eapply rtl_corestep_exec_Iop; eauto. simpl. reflexivity.
+
+exists mu. intuition.
+apply intern_incr_refl.
+apply sm_inject_separated_same_sminj.
+loc_alloc_solve.
+
+unfold MATCH; intuition.
+econstructor; eauto. apply match_stacks_inside_set_reg; auto. apply agree_set_reg; auto.
+(* without a result *)
+eexists. eexists.
+split; simpl. left.  
+eapply core_semantics_lemmas.corestep_plus_one. eapply rtl_corestep_exec_Inop; eauto.
+exists mu. intuition.
+apply intern_incr_refl.
+apply sm_inject_separated_same_sminj.
+apply sm_locally_allocatedChar.
+repeat split; extensionality b0;
+rewrite freshloc_irrefl;
+intuition.
+unfold MATCH; intuition.
+econstructor; eauto. subst vres. apply agree_set_reg_undef'; auto.
+Qed.
